Original_Dinitz_Algo.thy
@@ -1,9 +1,9 @@
 theory Original_Dinitz_Algo
-  imports Layering_Algo NetworkUtils (*EdmondsKarp_Maxflow.EdmondsKarp_Impl*) (*Refine_Monadic.Refine_Monadic*)
+  imports Graph_Restriction NetworkUtils Refine_Monadic.Refine_Monadic
 begin
 (* TODO do we need f? *)
 subsection \<open>Properties when removing a flow from the ST_Layering\<close>
-locale ST_Layered_Flow = NFlow c s t f + ST_Shortest_Path_Union stl cf s t + f': Flow stl s t f'
+locale ST_Layered_Flow = NFlow c s t f + Dual_Shortest_Path_Union stl cf s t + f': Flow stl s t f'
   for c s t f stl f'
 begin
 interpretation g': Irreducible_Graph stl
@@ -94,7 +94,7 @@ proof (unfold Graph.isPath_alt, clarify)
 qed
 
 lemma cleaning_maintains_bounded_union:
-  "Bounded_ST_Shortest_Path_Union (cleaning s t (g'.subtract_graph f')) (cf_of (augment f')) s t (cf.min_dist s t)"
+  "Bounded_Dual_Shortest_Path_Union (cleaning s t (g'.subtract_graph f')) (cf_of (augment f')) s t (cf.min_dist s t)"
 proof (cases "Graph.isEmpty f'")
   case True
   then have "(g'.subtract_graph f') = stl"
@@ -103,7 +103,7 @@ proof (cases "Graph.isEmpty f'")
     unfolding cleaning_def using g'.V_def g'.zero_cap_simp by fastforce
   moreover from True have "cf_of (augment f') = cf"
     unfolding Graph.isEmpty_def aug_cf_alt cf.subtract_skew_graph_def by simp
-  moreover note ST_Shortest_Path_Union_axioms
+  moreover note Dual_Shortest_Path_Union_axioms
   ultimately show ?thesis  by (simp add: min_st_dist_bound)
 next
   case False
@@ -111,7 +111,7 @@ next
     using f'.flow_pos_cont.edges_ss s_in_V_if_nonempty t_in_V_if_nonempty
     unfolding Graph.isEmpty_def by auto
   
-  show ?thesis unfolding Bounded_ST_Shortest_Path_Union_def Bounded_ST_Shortest_Path_Union_axioms_def
+  show ?thesis unfolding Bounded_Dual_Shortest_Path_Union_def Bounded_Dual_Shortest_Path_Union_axioms_def
   proof
     have "Subgraph (cleaning s t (g'.subtract_graph f')) (g'.subtract_graph f')"
       using cleaning_rp_Subgraph right_pass_Subgraph subgraph.order.trans by blast
@@ -210,7 +210,7 @@ thm Graph.subtract_path_alt
 definition dinitz_phase_invar :: "(_ flow \<times> _ graph) \<Rightarrow> bool" where
   "dinitz_phase_invar \<equiv> \<lambda>(f', stl).
     NFlow c s t f'
-    \<and> Bounded_ST_Shortest_Path_Union stl (cf_of f') s t (cf.min_dist s t)
+    \<and> Bounded_Dual_Shortest_Path_Union stl (cf_of f') s t (cf.min_dist s t)
     \<and> (Graph.connected (cf_of f') s t \<longrightarrow> (cf.min_dist s t) \<le> (Graph.min_dist (cf_of f') s t))"
 
 lemma dinitz_phase_step:
@@ -225,7 +225,7 @@ proof (intro conjI)
 
   have BOUND_EQ: "cf.min_dist s t = f'.cf.min_dist s t"
   proof -
-    from INVAR interpret Bounded_ST_Shortest_Path_Union stl f'.cf s t "cf.min_dist s t"
+    from INVAR interpret Bounded_Dual_Shortest_Path_Union stl f'.cf s t "cf.min_dist s t"
       unfolding dinitz_phase_invar_def by simp
     show ?thesis
     proof (intro antisym)
@@ -237,7 +237,7 @@ proof (intro conjI)
       by (metis Bounded_Shortest_Path_Union.obtain_close_ST Bounded_Shortest_Path_Union_axioms emptyE g'.isEmpty_def g'.isPath_bwd_cases min_dist_transfer s_in_V_if_nonempty singleton_iff t_not_s)
     qed
   qed
-  with INVAR interpret ST_Shortest_Path_Union stl f'.cf s t
+  with INVAR interpret Dual_Shortest_Path_Union stl f'.cf s t
     unfolding dinitz_phase_invar_def using min_st_dist_bound by fastforce
 
   interpret g': Nonnegative_Graph stl
@@ -290,7 +290,7 @@ proof (intro conjI)
   interpret st_layered_flow: ST_Layered_Flow c s t f' stl "f'.augmentingFlow p" by intro_locales
 
   have "NFlow c s t aug_f'" unfolding aug_f'_def using st_layered_flow.augment_NFlow .
-  moreover have "Bounded_ST_Shortest_Path_Union stl' (cf_of aug_f') s t (cf.min_dist s t)"
+  moreover have "Bounded_Dual_Shortest_Path_Union stl' (cf_of aug_f') s t (cf.min_dist s t)"
     using st_layered_flow.cleaning_maintains_bounded_union INDUCED_EQ BOUND_EQ
     unfolding g'.subtract_path_alt f'.augmentingFlow_alt aug_f'_def stl'_def by simp
   moreover have "(Graph.connected (cf_of aug_f') s t \<longrightarrow> cf.min_dist s t \<le> Graph.min_dist (cf_of aug_f') s t)"
@@ -325,10 +325,10 @@ proof
   from INVAR interpret f': NFlow c s t f' unfolding dinitz_phase_invar_def by blast
   show "NFlow c s t f'" using f'.NFlow_axioms .
 
-  from INVAR interpret Bounded_ST_Shortest_Path_Union stl f'.cf s t "cf.min_dist s t"
+  from INVAR interpret Bounded_Dual_Shortest_Path_Union stl f'.cf s t "cf.min_dist s t"
     unfolding dinitz_phase_invar_def by blast
   from DISCON show "f'.cf.connected s t \<longrightarrow> cf.min_dist s t < f'.cf.min_dist s t"
-    by (metis Bounded_ST_Shortest_Path_Union_axioms ST_Shortest_Path_Union.st_connected_iff le_eq_less_or_eq linorder_neqE_nat min_st_dist_bound)
+    by (metis Bounded_Dual_Shortest_Path_Union_axioms Dual_Shortest_Path_Union.st_connected_iff le_eq_less_or_eq linorder_neqE_nat min_st_dist_bound)
 qed
 
 lemma dinitz_phase_correct:
@@ -385,582 +385,5 @@ theorem dinitz_correct: "dinitz \<le> SPEC (\<lambda>f. isMaxFlow f)"
   by (simp add: Graph.connected_def Graph.isSimplePath_def NFlow.axioms(1) NFlow.ford_fulkerson(1) NPreflow.isAugmentingPath_def)
 end
 
-subsection \<open>Dinitz phase refinement\<close>
-context Graph
-begin
-(* TODO bounded version *)
-definition build_st_layering :: "node \<Rightarrow> node \<Rightarrow> _ graph nres" where
-  "build_st_layering s t \<equiv> do {
-    sl \<leftarrow> ebfs s;
-    stl \<leftarrow> Graph.back_ebfs sl t;
-    RETURN stl
-  }"
-end
 
-(* TODO is Finite_Graph really what we want? *)
-context Finite_Graph
-begin
-lemma build_st_layering_correct:
-  "build_st_layering s t \<le> (spec c'. ST_Shortest_Path_Union c' c s t)"
-  unfolding build_st_layering_def
-proof (refine_vcg, simp)
-  have "reachableNodes s \<subseteq> V \<union> {s}"
-    using Graph.distinct_nodes_in_V_if_connected(2) reachableNodes_def by auto
-  then have "finite (reachableNodes s)" using finite_V by (simp add: finite_subset)
-  then have "ebfs s \<le> (spec sl. S_Shortest_Path_Union sl c s V)" by (rule ebfs_correct)
-  also have "... \<le> (spec sl. Graph.back_ebfs sl t \<le> (spec c'. ST_Shortest_Path_Union c' c s t))"
-  proof (rule SPEC_rule)
-    fix c'
-    assume "S_Shortest_Path_Union c' c s V"
-    then interpret S_Shortest_Path_Union c' c s V .
-
-    have "{u. g'.connected u t} \<subseteq> V' \<union> {t}"
-      using g'.distinct_nodes_in_V_if_connected by auto
-    then have "finite {u. g'.connected u t}" using finite_V V_ss by (simp add: finite_subset)
-    then have "g'.back_ebfs t \<le> (spec c''. T_Shortest_Path_Union c'' c' V' t)"
-      by (rule g'.back_ebfs_correct)
-    also from \<open>S_Shortest_Path_Union c' c s V\<close> have "... \<le> (spec c''. ST_Shortest_Path_Union c'' c s t)"
-      using SPEC_rule ST_SPU_dualI by metis
-    finally show "g'.back_ebfs t \<le> (spec c''. ST_Shortest_Path_Union c'' c s t)" .
-  qed
-  finally show "ebfs s \<le> (spec sl. Graph.back_ebfs sl t \<le> (spec c'. ST_Shortest_Path_Union c' c s t))" .
-qed
-
-end
-
-
-
-context NFlow
-begin
-
-section \<open>Experiment\<close>
-definition test1 :: "_ flow nres" where
-  "test1 \<equiv> do {
-    (f', _, _) \<leftarrow> WHILE\<^sub>T
-      (\<lambda>(_, _, brk). \<not> brk)
-      (\<lambda>(f', stl, _). do {
-            stl \<leftarrow> Graph.subtract_path_algo stl [(0, 0)];
-            RETURN (f', stl, False)
-          })
-      (f, c, False);
-    RETURN f'}"
-definition test2 :: "_ flow nres" where
-  "test2 \<equiv> do {
-    (f', _, _) \<leftarrow> WHILE\<^sub>T
-      (\<lambda>(_, _, brk). \<not> brk)
-      (\<lambda>(f', stl, _). do {
-            stl \<leftarrow> return (Graph.subtract_path stl [(0, 0)]);
-            RETURN (f', stl, False)
-          })
-      (f, c, False);
-    RETURN f'}"
-
-thm refine_dref_pattern
-(* TODO find out which rule leads to the spec term, which in turn means dref_type cannot infer relation type *)
-lemma "test1 \<le> \<Down> Id test2"
-  unfolding test1_def test2_def
-  apply refine_rcg
-         apply refine_dref_type
-      apply clarsimp_all
-  oops
-\<comment> \<open>Experiment\<close>
-
-
-
-
-
-(* TODO *)
-(*declare fun_relI[refine del]*)
-lemma RELATESI_workaround[refine_dref_pattern]:
-  "RELATES R \<Longrightarrow> S \<le> (spec x. (x, y) \<in> R) \<Longrightarrow> S \<le> (spec x. (x, y) \<in> R)" .
-
-
-thm build_st_layering_correct
-  ST_Layer_Graph.greedy_st_path_finding_correct
-  subtract_path_algo_correct
-  Graph.inner_path_vertices_algo_correct
-  Finite_Bounded_Graph.cleaning_algo_correct
-
-(* TODO cleanup assertions *)
-
-(*
-definition dinitz_phase_assert_invar :: "(_ flow \<times> _ graph \<times> bool) \<Rightarrow> bool" where
-  "dinitz_phase_assert_invar \<equiv> \<lambda>(f', stl, brk).
-    NFlow c s t f'
-    \<and> Bounded_ST_Shortest_Path_Union stl (cf_of f') s t (cf.min_dist s t)
-    \<and> (Graph.connected (cf_of f') s t \<longrightarrow> cf.min_dist s t \<le> Graph.min_dist (cf_of f') s t)
-    \<and> (brk \<longrightarrow> \<not> Graph.connected stl s t)"
-
-definition dinitz_phase_assert :: "_ flow nres" where
-  "dinitz_phase_assert \<equiv> do {
-    stl \<leftarrow> (spec c'. ST_Shortest_Path_Union c' cf s t);
-    (f', _, _) \<leftarrow> WHILE\<^sub>T\<^bsup>dinitz_phase_assert_invar\<^esup>
-      (\<lambda>(_, _, brk). \<not> brk)
-      (\<lambda>(f', stl, _). do {
-        p' \<leftarrow> select p. Graph.isPath stl s p t;
-        case p' of
-          None \<Rightarrow> RETURN (f', stl, True)
-        | Some p \<Rightarrow> do {
-            assert (Graph.isPath stl s p t);
-            assert (ST_Shortest_Path_Union stl (cf_of f') s t);
-            Q_ls \<leftarrow> return (tl (butlast (Graph.pathVertices s p)));
-            assert (set Q_ls = set (Graph.pathVertices s p) - {s, t});
-            stl' \<leftarrow> return (Graph.subtract_path stl p);
-            assert (Contained_Graph stl' stl \<and> Graph.E stl \<subseteq> Graph.E stl' \<union> set p);
-            stl' \<leftarrow> return (cleaning s t stl');
-            let f' = NFlow.augment c f' (NPreflow.augmentingFlow c f' p);
-            RETURN (f', stl', False)
-          }})
-      (f, stl, False);
-    RETURN f'}"
-*)
-
-definition dinitz_phase_assert_invar :: "(_ flow \<times> _ graph \<times> bool \<times> bool) \<Rightarrow> bool" where
-  "dinitz_phase_assert_invar \<equiv> \<lambda>(f', stl, brk, changed).
-    NFlow c s t f'
-    \<and> Bounded_ST_Shortest_Path_Union stl (cf_of f') s t (cf.min_dist s t)
-    \<and> (Graph.connected (cf_of f') s t \<longrightarrow> cf.min_dist s t \<le> Graph.min_dist (cf_of f') s t)
-    \<and> (brk \<longrightarrow> \<not> Graph.connected stl s t)
-    \<and> (val \<le> Flow.val c s f')
-    \<and> (changed \<longleftrightarrow> f' \<noteq> f)
-    \<and> (changed \<longrightarrow> cf.connected s t)" (* \<and> (changed \<and> brk \<longrightarrow> cf.connected s t)" *)
-
-(* TODO can this be simplified to just changed \<longleftrightarrow> val < val'? *)
-lemma dinitz_phase_assert_invar_alt:
-  "dinitz_phase_assert_invar = (\<lambda>(f', stl, brk, changed).
-    dinitz_phase_invar (f', stl)
-    \<and> (brk \<longrightarrow> \<not> Graph.connected stl s t)
-    \<and> (val \<le> Flow.val c s f')
-    \<and> (changed \<longleftrightarrow> f' \<noteq> f)
-    \<and> (changed \<longrightarrow> cf.connected s t))" (* TODO does this work? *)
-  unfolding dinitz_phase_invar_def dinitz_phase_assert_invar_def by simp
-
-definition dinitz_phase_assert :: "(_ flow \<times> bool) nres" where
-  "dinitz_phase_assert \<equiv> do {
-    stl \<leftarrow> (spec c'. ST_Shortest_Path_Union c' cf s t);
-    (f', _, _, changed) \<leftarrow> WHILE\<^sub>T\<^bsup>dinitz_phase_assert_invar\<^esup>
-      (\<lambda>(_, _, brk, _). \<not> brk)
-      (\<lambda>(f', stl, _, changed). do {
-        p' \<leftarrow> select p. Graph.isPath stl s p t;
-        case p' of
-          None \<Rightarrow> RETURN (f', stl, True, changed)
-        | Some p \<Rightarrow> do {
-            assert (Graph.isPath stl s p t);
-            assert (ST_Shortest_Path_Union stl (cf_of f') s t);
-            Q_ls \<leftarrow> return (tl (butlast (Graph.pathVertices s p)));
-            assert (set Q_ls = set (Graph.pathVertices s p) - {s, t});
-            stl' \<leftarrow> return (Graph.subtract_path stl p);
-            assert (Contained_Graph stl' stl \<and> Graph.E stl \<subseteq> Graph.E stl' \<union> set p);
-            stl' \<leftarrow> return (cleaning s t stl');
-            let f' = NFlow.augment c f' (NPreflow.augmentingFlow c f' p);
-            RETURN (f', stl', False, True)
-          }})
-      (f, stl, False, False);
-    RETURN (f', changed)}"
-
-(* TODO comment about val needed for changed inequality *)
-
-(* TODO use this in phase step *)
-lemma stu_if_invar_and_path:
-  assumes INVAR: "dinitz_phase_invar (f', stl)"
-    and PATH: "Graph.isPath stl s p t"
-  shows "ST_Shortest_Path_Union stl (cf_of f') s t"
-proof -
-  from INVAR interpret f': NFlow c s t f' unfolding dinitz_phase_invar_def by blast
-
-  have BOUND_EQ: "cf.min_dist s t = f'.cf.min_dist s t"
-  proof -
-    from INVAR interpret Bounded_ST_Shortest_Path_Union stl f'.cf s t "cf.min_dist s t"
-      unfolding dinitz_phase_invar_def by simp
-    show ?thesis
-    proof (intro antisym)
-      from PATH INVAR show "cf.min_dist s t \<le> f'.cf.min_dist s t"
-        unfolding dinitz_phase_invar_def Graph.connected_def
-        using sg_paths_are_base_paths by blast
-      from PATH show "f'.cf.min_dist s t \<le> cf.min_dist s t" (* TODO fix proof *)
-      using f'.cf.isShortestPath_min_dist_def path_length_bounded shortest_path_transfer (* by simp *)
-      by (metis Bounded_Shortest_Path_Union.obtain_close_ST Bounded_Shortest_Path_Union_axioms emptyE g'.isEmpty_def g'.isPath_bwd_cases min_dist_transfer s_in_V_if_nonempty singleton_iff t_not_s)
-    qed
-  qed
-  with INVAR show "ST_Shortest_Path_Union stl (f'.cf) s t"
-    unfolding dinitz_phase_invar_def using min_st_dist_bound by fastforce
-qed
-
-lemma dinitz_phase_assert_step:
-  fixes f' stl changed
-  assumes PATH: "Graph.isPath stl s p t"
-      and INVAR: "dinitz_phase_assert_invar (f', stl, False, changed)"
-  defines "aug_f' \<equiv> NFlow.augment c f' (NPreflow.augmentingFlow c f' p)"
-      and "stl' \<equiv> cleaning s t (Graph.subtract_path stl p)"
-    shows "dinitz_phase_assert_invar (aug_f', stl', False, True) \<and> Graph.E stl' \<subset> Graph.E stl \<and> finite (Graph.E stl)"
-proof -
-  have "Flow.val c s f' < Flow.val c s aug_f'"
-  proof -
-    from INVAR interpret f': NFlow c s t f' unfolding dinitz_phase_assert_invar_def by blast
-    from INVAR PATH interpret stu: ST_Shortest_Path_Union stl "cf_of f'" s t
-      unfolding dinitz_phase_assert_invar_alt using stu_if_invar_and_path by blast
-
-    have "Flow f'.cf s t (f'.augmentingFlow p)"
-      apply (intro f'.augFlow_resFlow)
-      unfolding f'.isAugmentingPath_def
-      using PATH f'.cf.isShortestPath_alt stu.shortest_path_transfer by blast
-    moreover have "0 < Flow.val f'.cf s (f'.augmentingFlow p)"
-      by (simp add: Graph.shortestPath_is_path Graph.shortestPath_is_simple PATH f'.augFlow_val f'.isAugmentingPath_def f'.resCap_gzero_aux stu.shortest_path_transfer)
-    ultimately show ?thesis unfolding aug_f'_def using f'.augment_flow_value by simp
-  qed
-  with PATH INVAR show ?thesis unfolding dinitz_phase_assert_invar_alt aug_f'_def stl'_def
-    using dinitz_phase_step (* TODO prettify *)
-    apply auto
-    apply (meson Graph.connected_def ST_Shortest_Path_Union.st_connected_iff stu_if_invar_and_path)
-    by blast+
-qed
-
-
-
-
-definition "dinitz_phase_assert_wf_rel \<equiv> inv_image
-  (less_than_bool <*lex*> finite_psubset)
-  (\<lambda>(_, stl, brk, _). (\<not>brk, Graph.E stl))"
-
-
-find_theorems Graph.E Graph.subtract_path
-find_theorems Graph.E Graph.subtract_graph
-thm Graph.subtract_graph_untouched_edges
-
-lemma dinitz_phase_assert_correct:
-  "dinitz_phase_assert \<le> SPEC (\<lambda>(f', changed). res_dist_increasing_flow f' \<and> changed = (f' \<noteq> f) \<and> (changed \<longrightarrow> cf.connected s t))"
-  unfolding dinitz_phase_assert_def
-  apply (refine_vcg WHILEIT_rule[where R=dinitz_phase_assert_wf_rel])
-                      apply (all \<open>(clarsimp; fail)?\<close>)
-            apply (simp add: dinitz_phase_assert_wf_rel_def wf_lex_prod)
-            apply (simp add: dinitz_phase_assert_invar_def NFlow_axioms min_st_dist_bound)
-           defer defer defer
-  apply (simp add: Graph.subtract_path_alt) using Graph.subtract_graph_untouched_edges apply (metis (no_types, lifting) Graph.isPath_alt Graph.path_induced_graph_edges Int_Un_eq(4) Int_absorb1 Int_commute Un_Diff_cancel2 cf.isPath.simps(1) set_eq_subset t_not_s)
-          apply (simp add: dinitz_phase_assert_step)
-          apply (simp add: dinitz_phase_assert_step dinitz_phase_assert_wf_rel_def)
-        apply (simp add: dinitz_phase_assert_invar_alt Graph.connected_def)
-       apply (simp add: dinitz_phase_assert_wf_rel_def)
-      apply (clarsimp simp: dinitz_phase_assert_invar_alt dinitz_phase_final)
-      apply (simp add: dinitz_phase_assert_invar_alt)
-  apply (clarsimp simp: dinitz_phase_assert_invar_alt)
-proof clarsimp_all
-  fix f' stl p changed
-  interpret cf': Graph "cf_of f'" .
-  assume INVAR: "dinitz_phase_assert_invar (f', stl, False, changed)" and PATH: "Graph.isPath stl s p t"
-  then show "ST_Shortest_Path_Union stl (cf_of f') s t"
-    unfolding dinitz_phase_assert_invar_alt using stu_if_invar_and_path by blast
-  then interpret ST_Shortest_Path_Union stl "cf_of f'" s t .
-
-  from INVAR interpret f': NFlow c s t f' unfolding dinitz_phase_assert_invar_def by blast
-  interpret g': Nonnegative_Graph stl
-    using f'.cf.Nonnegative_Graph_axioms sg_Nonnegative_Graph by blast
-  (* TODO replace this with a simple 'have', need some way to use sublocale relations *)
-  interpret subt_pos_cont: Pos_Contained_Graph "g'.subtract_path p" stl
-    unfolding g'.subtract_path_alt
-    using g'.path_induced_graph_pos_contained Pos_Contained_Graph.subtract_le_contained by blast
-  show "Contained_Graph (g'.subtract_path p ) stl" by intro_locales
-
-  from PATH have "pathVertices s p = s # (tl (pathVertices s p))"
-    by (simp add: Graph.pathVertices_fwd pathVertices_fwd_def)
-  moreover from PATH have "pathVertices s p = butlast (pathVertices s p) @ [t]"
-    by (metis Graph.isPath_bwd_cases Graph.isPath_tail Graph.pathVertices_alt snoc_eq_iff_butlast' t_not_s)
-  ultimately have "pathVertices s p = s # (tl (butlast (pathVertices s p))) @ [t]"
-    by (metis butlast_tl empty_append_eq_id snoc_eq_iff_butlast' t_not_s tl_last)
-      (* TODO simplify, probably need to show s, t \<notin> tl (butlast (pathVertices s p)) *)
-  then show "set (tl (butlast (pathVertices s p))) = set (pathVertices s p) - {s, t}"
-    by (smt (verit, ccfv_threshold) Diff_insert0 Graph.isSimplePath_fwd Graph.pathVertices_fwd PATH Un_Diff_Int Un_insert_right distinct.simps(2) distinct_append empty_set insertCI insert_Diff1 list.simps(15) paths_are_simple set_append sup_bot.right_neutral)
-qed
-
-definition dinitz_phase_concrete :: "(_ flow \<times> bool) nres" where
-  "dinitz_phase_concrete \<equiv> do {
-    stl \<leftarrow> cf.build_st_layering s t;
-    (f', _, _, changed) \<leftarrow> WHILE\<^sub>T\<^bsup>dinitz_phase_assert_invar\<^esup>
-      (\<lambda>(_, _, brk, _). \<not> brk)
-      (\<lambda>(f', stl, _, changed). do {
-        p' \<leftarrow> Graph.greedy_st_path_finding stl s t;
-        case p' of
-          None \<Rightarrow> RETURN (f', stl, True, changed)
-        | Some p \<Rightarrow> do {
-            assert (Graph.isPath stl s p t);
-            assert (ST_Shortest_Path_Union stl (cf_of f') s t);
-            Q_ls \<leftarrow> inner_path_vertices_algo p;
-            assert (set Q_ls = set (Graph.pathVertices s p) - {s, t});
-            stl' \<leftarrow> Graph.subtract_path_algo stl p;
-            assert (Contained_Graph stl' stl \<and> Graph.E stl \<subseteq> Graph.E stl' \<union> set p);
-            stl' \<leftarrow> cleaning_algo (set Q_ls) stl';
-            let f' = NFlow.augment c f' (NPreflow.augmentingFlow c f' p);
-            RETURN (f', stl', False, True)
-          }})
-      (f, stl, False, False);
-    RETURN (f', changed)}"
-
-
-
-
-
-find_theorems Graph.pathVertices set
-find_theorems Graph.pathVertices_fwd set
-find_theorems Graph.pathVertices
-thm Graph.pathVertices_append
-
-(*
-lemma (in Graph) aux: "u \<notin> set (pathVertices s p) \<Longrightarrow> (u, v) \<notin> set p"
-  by (induction p arbitrary: s) auto(*TODO*)
-lemma (in Graph) aux2: "u \<notin> set (pathVertices s p) \<Longrightarrow> (v, u) \<notin> set p"
-  apply (induction p arbitrary: s)
-   apply simp
-  apply simp sledgehammer
-  apply (induction p arbitrary: s rule: rev_induct)
-   apply simp
-  apply (simp add: Graph.pathVertices_append) apply auto
-  by (induction p arbitrary: s) auto(*TODO*)*)
-
-
-
-lemma dinitz_phase_concrete_refine: "dinitz_phase_concrete \<le> \<Down> Id dinitz_phase_assert"
-  unfolding dinitz_phase_concrete_def dinitz_phase_assert_def
-  apply refine_rcg
-            apply refine_dref_type
-           apply clarsimp_all
-  using cf.build_st_layering_correct apply simp
-proof -
-  fix f' stl changed
-  assume "dinitz_phase_assert_invar (f', stl, False, changed)"
-  then interpret bstu: Bounded_ST_Shortest_Path_Union stl "cf_of f'" s t "cf.min_dist s t"
-    unfolding dinitz_phase_assert_invar_def by blast
-  show "Graph.greedy_st_path_finding stl s t \<le> (select p. Graph.isPath stl s p t)"
-    using bstu.greedy_st_path_finding_correct .
-next
-  fix f' stl p
-  assume "ST_Shortest_Path_Union stl (cf_of f') s t"
-  then interpret stu: ST_Shortest_Path_Union stl "cf_of f'" s t .
-
-  assume "Graph.isPath stl s p t"
-  then have SP: "Graph.isPath stl s p t" by blast
-  
-  show "inner_path_vertices_algo p \<le> RES {tl (butlast (Graph.pathVertices s p))}"
-    using inner_path_vertices_algo_correct by (simp add: RES_sng_eq_RETURN)
-
-  from SP show "Graph.subtract_path_algo stl p \<le> RES {Graph.subtract_path stl p}"
-    using stu.g'.isSPath_distinct stu.paths_are_simple stu.g'.subtract_path_algo_correct
-    by (metis RES_sng_eq_RETURN)
-
-  thm Finite_Bounded_Graph.cleaning_algo_correct
-  fix stl'
-  assume "Contained_Graph stl' stl" "Graph.E stl \<subseteq> Graph.E stl' \<union> set p"
-  show "cleaning_algo (set (Graph.pathVertices s p) - {s, t}) stl' \<le> RES {cleaning s t stl'}"
-  proof (unfold RES_sng_eq_RETURN, intro Finite_Bounded_Graph.cleaning_algo_correct)
-    show "s \<notin> set (Graph.pathVertices s p) - {s, t}"
-      "t \<notin> set (Graph.pathVertices s p) - {s, t}"
-      "finite (set (Graph.pathVertices s p) - {s, t})"
-      by auto
-    from \<open>Contained_Graph stl' stl\<close> show "Finite_Bounded_Graph stl' (stu.layer t)" unfolding Finite_Bounded_Graph_def
-      by (meson Finite_Graph.intro Graph.Efin_imp_Vfin Contained_Graph.edges_ss Contained_Graph.cont_Distance_Bounded cfE_of_finite infinite_super stu.Distance_Bounded_Graph_axioms stu.E'_ss)
-    from \<open>Contained_Graph stl' stl\<close> show "Graph.incoming stl' s = {}"
-      by (metis Graph.isShortestPath_min_dist_def SP Contained_Graph.cont_incoming_ss bot.extremum_uniqueI stu.b_length_paths_are_terminal(1) stu.path_is_shortest)
-      (*by (metis Subgraph.incoming_ss Subgraph_axioms incoming_s_empty subset_empty)*)
-    from \<open>Contained_Graph stl' stl\<close> show "Graph.outgoing stl' t = {}"
-      by (metis Diff_empty Diff_eq_empty_iff Graph.distinct_nodes_in_V_if_connected(2) Contained_Graph.cont_outgoing_ss stu.no_outgoingD stu.obtain_back_terminal_connected)
-      (*by (metis Subgraph.outgoing_ss Subgraph_axioms outgoing_t_empty subset_empty)*)
-    from \<open>Graph.E stl \<subseteq> Graph.E stl' \<union> set p\<close> show "\<forall>u\<in>Graph.V stl' - (set (Graph.pathVertices s p) - {s, t}) - {s, t}. Graph.incoming stl' u \<noteq> {} \<and> Graph.outgoing stl' u \<noteq> {}"
-    proof auto (* TODO *)
-      fix v
-      assume "v \<in> Graph.V stl'"
-      then have "v \<in> Graph.V stl" using Contained_Graph.vertices_ss[OF \<open>Contained_Graph stl' stl\<close>] by blast
-      moreover assume "v \<noteq> s" "v \<noteq> t"
-      ultimately obtain u w where IN_OUT: "(u, v) \<in> Graph.E stl" "(v, w) \<in> Graph.E stl"
-        by (metis Graph.isPath_bwd_cases Graph.isPath_fwd_cases stu.g'.connected_def stu.st_connected)
-      
-      assume "v \<notin> set (Graph.pathVertices s p)"
-      with \<open>Graph.isPath stl s p t\<close> have "v \<notin> set (Graph.pathVertices_fwd s p)"
-        by (simp add: stu.g'.pathVertices_fwd)
-      from IN_OUT have "(u, v) \<notin> set p" "(v, w) \<notin> set p" using stu.g'.adjacent_edges_not_on_path[OF \<open>Graph.isPath stl s p t\<close> \<open>v \<notin> set (Graph.pathVertices_fwd s p)\<close>]
-        unfolding stu.g'.adjacent_def stu.g'.incoming_def stu.g'.outgoing_def by auto
-      with \<open>Graph.E stl \<subseteq> Graph.E stl' \<union> set p\<close> IN_OUT have "(u, v) \<in> Graph.E stl'" "(v, w) \<in> Graph.E stl'" by auto
-      then show "Graph.incoming stl' v = {} \<Longrightarrow> False" "Graph.outgoing stl' v = {} \<Longrightarrow> False"
-        unfolding Graph.incoming_def Graph.outgoing_def by auto
-    qed
-  qed
-qed
-
-lemma dinitz_phase_concrete_correct: "dinitz_phase_concrete \<le> SPEC (\<lambda>(f', changed). res_dist_increasing_flow f' \<and> changed = (f' \<noteq> f) \<and> (changed \<longrightarrow> cf.connected s t))"
-  using dinitz_phase_concrete_refine dinitz_phase_assert_correct by simp
-end
-
-context Network
-begin
-(* TODO rework using changed flag *)
-definition dinitz_concrete :: "_ flow nres" where
-  "dinitz_concrete \<equiv> do {
-    (f, _) \<leftarrow> WHILE\<^sub>T snd (NFlow.dinitz_phase_concrete c s t \<circ> fst) (\<lambda>_. 0, True);
-    RETURN f}"
-
-(*
-definition dinitz_concrete_aux_rel where
-  "dinitz_concrete_aux_rel \<equiv> {((f, m), f)|f m. m \<or> isMaxFlow f}"
-term dinitz_concrete_aux_rel
-thm dinitz_concrete_aux_rel_def
-
-thm bind_refine
-lemma dinitz_concrete_refine: "dinitz_concrete \<le> \<Down> Id dinitz"
-  unfolding dinitz_concrete_def dinitz_def
-  apply (refine_rcg bind_refine[where R'=dinitz_concrete_aux_rel])
-  unfolding dinitz_concrete_aux_rel_def apply clarsimp_all
-  defer using NFlow.dinitz_phase_concrete_refine apply clarsimp
-*)
-find_consts "('a \<Rightarrow> bool) \<Rightarrow> ('b \<Rightarrow> bool) \<Rightarrow> 'a \<times> 'b \<Rightarrow> bool"
-term pred_prod
-
-
-theorem dinitz_concrete_correct: "dinitz_concrete \<le> SPEC (\<lambda>f. isMaxFlow f)"
-  unfolding dinitz_concrete_def
-  apply (refine_vcg WHILET_rule[where I="\<lambda>(f', m). NFlow c s t f' \<and> (m \<or> isMaxFlow f')"
-          and R="inv_image (less_than_bool <*lex*> res_dist_rel) prod.swap"])
-      apply (fastforce simp: res_dist_wf)
-     apply (clarsimp_all simp: NFlowI Network_axioms zero_is_flow)
-proof -
-  fix f
-  assume "NFlow c s t f"
-  then interpret NFlow c s t f .
-  have "dinitz_phase_concrete \<le> SPEC (\<lambda>(f', changed). res_dist_increasing_flow f' \<and> changed = (f' \<noteq> f) \<and> (changed \<longrightarrow> cf.connected s t))"
-    using dinitz_phase_concrete_correct .
-  also have "... \<le> (spec s'. (case s' of (f', m) \<Rightarrow> NFlow c s t f' \<and> (m \<or> isMaxFlow f')) \<and> (prod.swap s', True, f) \<in> less_than_bool <*lex*> res_dist_rel)"
-  proof (clarsimp, intro conjI)
-    fix f'
-    assume "res_dist_increasing_flow f'" and CON_IF_NEQ: "(f' \<noteq> f) \<longrightarrow> cf.connected s t"
-    then show "NFlow c s t f'"
-      unfolding res_dist_increasing_flow_def by simp
-    then interpret n': NFlow c s t f' .
-    from \<open>res_dist_increasing_flow f'\<close> have DIST: "n'.cf.connected s t \<longrightarrow> cf.min_dist s t < n'.cf.min_dist s t"
-      unfolding res_dist_increasing_flow_def by simp
-    with CON_IF_NEQ show "f' = f \<or> f' \<noteq> f \<and> (f', f) \<in> res_dist_rel" unfolding res_dist_rel_def by blast
-    from CON_IF_NEQ show "f' = f \<longrightarrow> isMaxFlow f"
-      using Graph.connected_def Graph.isSimplePath_fwd n'.fofu_III_I n'.fofu_II_III n'.isAugmentingPath_def DIST by blast
-  qed 
-  finally show "dinitz_phase_concrete \<le> (spec s'. (case s' of (f', m) \<Rightarrow> NFlow c s t f' \<and> (m \<or> isMaxFlow f')) \<and> (prod.swap s', True, f) \<in> less_than_bool <*lex*> res_dist_rel)" .
-qed
-
-(*
-term SPEC
-term "if changed then cf.connected s t \<and> res_dist_increasing_flow f' else \<not> cf.connected s t \<and> (f' = f))"
-lemma (in NFlow) dinitz_phase_concrete_correct_if:
-  "dinitz_phase_concrete \<le> SPEC (\<lambda>(f', changed).
-    (if changed then cf.connected s t \<and> res_dist_increasing_flow f' else \<not> cf.connected s t \<and> (f' = f)))"
-
-
-res_dist_increasing_flow f' \<and> changed = (cf.connected s t \<and> f' \<noteq> f))"
-  sorry*)
-
-
-
-(*
-term "inv_image (less_than_bool <*lex*> res_dist_rel) prod.swap"
-theorem dinitz_concrete_correct: "dinitz_concrete \<le> SPEC (\<lambda>f. isMaxFlow f)"
-  unfolding dinitz_concrete_def
-  apply (refine_vcg WHILET_rule[where I="\<lambda>(f', m). NFlow c s t f' \<and> (m \<or> isMaxFlow f')"
-          and R="inv_image (less_than_bool <*lex*> res_dist_rel) prod.swap"])
-      apply (fastforce simp: res_dist_wf)
-     apply (simp add: NFlowI Network_axioms zero_is_flow)
-    apply simp
-   defer apply simp
-
-proof clarsimp
-  fix f
-  assume "NFlow c s t f"
-  then interpret n: NFlow c s t f .
-  thm n.dinitz_phase_concrete_correct
-  have "n.dinitz_phase_concrete \<le> SPEC (\<lambda>(f', changed). n.res_dist_increasing_flow f' \<and> changed = (f' \<noteq> f))"
-    using n.dinitz_phase_concrete_correct .
-  also have "... \<le> (spec s'. (case s' of (f', m) \<Rightarrow> NFlow c s t f' \<and> (m \<or> isMaxFlow f')) \<and> (prod.swap s', True, f) \<in> less_than_bool <*lex*> res_dist_rel)"
-  proof (clarsimp, intro conjI)
-    fix f'
-    assume "n.res_dist_increasing_flow f'"
-    then show "NFlow c s t f'"
-      unfolding n.res_dist_increasing_flow_def by simp
-    then interpret n': NFlow c s t f' .
-    from \<open>n.res_dist_increasing_flow f'\<close> have DIST: "n'.cf.connected s t \<longrightarrow> n.cf.min_dist s t < n'.cf.min_dist s t"
-      unfolding n.res_dist_increasing_flow_def by simp
-
-    then show "NFlow c s t f' \<and> (f' = f \<longrightarrow> isMaxFlow f) \<and> (f' = f \<or> f' \<noteq> f \<and> (f', f) \<in> res_dist_rel)"
-      unfolding n.res_dist_increasing_flow_def apply auto
-        apply (meson Graph.connected_def Graph.isSimplePath_fwd n.ford_fulkerson(1) n.isAugmentingPath_def)
-      unfolding res_dist_rel_def apply auto oops
-
-
-      thm res_dist_rel_def
-
-theorem dinitz_concrete_correct: "dinitz_concrete \<le> SPEC (\<lambda>f. isMaxFlow f)"
-  unfolding dinitz_concrete_def
-  apply (refine_vcg WHILET_rule[where I="\<lambda>(f', m). NFlow c s t f' \<and> (m \<or> isMaxFlow f')"
-          and R="inv_image (less_than_bool <*lex*> res_dist_rel) prod.swap"])
-      apply (fastforce simp: res_dist_wf)
-     apply (simp add: NFlowI Network_axioms zero_is_flow)
-    apply simp
-   defer apply simp
-
-proof clarsimp
-  fix f
-  assume "NFlow c s t f"
-  then interpret n: NFlow c s t f .
-  thm n.dinitz_phase_concrete_correct'
-  have "n.dinitz_phase_concrete \<le> SPEC (\<lambda>(f', changed). n.res_dist_increasing_flow f' \<and> (changed \<longleftrightarrow> n.val < Flow.val c s f'))"
-    using n.dinitz_phase_concrete_correct' sorry
-  also have "... \<le> (spec s'. (case s' of (f', m) \<Rightarrow> NFlow c s t f' \<and> (m \<or> isMaxFlow f')) \<and> (prod.swap s', True, f) \<in> less_than_bool <*lex*> res_dist_rel)"
-  proof (clarsimp, intro conjI)
-    fix f'
-    assume "n.res_dist_increasing_flow f'"
-    then show "NFlow c s t f'"
-      unfolding n.res_dist_increasing_flow_def by simp
-    then interpret n': NFlow c s t f' .
-
-    from \<open>n.res_dist_increasing_flow f'\<close> have DIST: "n'.cf.connected s t \<longrightarrow> n.cf.min_dist s t < n'.cf.min_dist s t"
-      unfolding n.res_dist_increasing_flow_def by simp
-    then show "n.val < n'.val \<or> isMaxFlow f'" apply auto
-       apply (simp add: n'.ford_fulkerson(1) Graph.connected_def Graph.isSimplePath_fwd n'.isAugmentingPath_def)
-      sorry
-
-    from DIST show "n.val < n'.val \<longrightarrow> (f', f) \<in> res_dist_rel"
-      unfolding res_dist_rel_def
-      apply auto
-      by (meson Graph.connected_def Graph.isSimplePath_fwd isMaxFlow_def less_le_not_le n'.Flow_axioms n.fofu_III_I n.fofu_II_III n.isAugmentingPath_def)+
-
-    oops
-
-theorem dinitz_concrete_correct: "dinitz_concrete \<le> SPEC (\<lambda>f. isMaxFlow f)"
-  unfolding dinitz_concrete_def
-  apply (refine_vcg WHILET_rule[where I="\<lambda>(f', m). NFlow c s t f' \<and> (m \<or> isMaxFlow f')"
-          and R="inv_image (less_than_bool <*lex*> res_dist_rel) prod.swap"])
-      apply (fastforce simp: res_dist_wf)
-     apply (simp add: NFlowI Network_axioms zero_is_flow)
-    apply simp
-   defer apply simp
-
-proof clarsimp
-  fix f
-  assume "NFlow c s t f"
-  then interpret n: NFlow c s t f .
-  thm n.dinitz_phase_concrete_correct'
-  have "n.dinitz_phase_concrete \<le> SPEC (\<lambda>(f', changed). n.res_dist_increasing_flow f' \<and> (changed \<or> f' = f \<and> isMaxFlow f))"
-    using n.dinitz_phase_concrete_correct' .
-  also have "... \<le> (spec s'. (case s' of (f', m) \<Rightarrow> NFlow c s t f' \<and> (m \<or> isMaxFlow f')) \<and> (prod.swap s', True, f) \<in> less_than_bool <*lex*> res_dist_rel)"
-  proof (clarsimp, intro conjI)
-    fix f'
-    assume "n.res_dist_increasing_flow f'"
-    then show "NFlow c s t f'"
-      unfolding n.res_dist_increasing_flow_def by simp
-    then interpret n': NFlow c s t f' .
-
-    from \<open>n.res_dist_increasing_flow f'\<close> have DIST: "n'.cf.connected s t \<longrightarrow> n.cf.min_dist s t < n'.cf.min_dist s t"
-      unfolding n.res_dist_increasing_flow_def by simp
-    then show "n.val < n'.val \<or> isMaxFlow f'" apply auto
-       apply (simp add: n'.ford_fulkerson(1) Graph.connected_def Graph.isSimplePath_fwd n'.isAugmentingPath_def)
-      sorry
-
-    from DIST show "n.val < n'.val \<longrightarrow> (f', f) \<in> res_dist_rel"
-      unfolding res_dist_rel_def
-      apply auto
-      by (meson Graph.connected_def Graph.isSimplePath_fwd isMaxFlow_def less_le_not_le n'.Flow_axioms n.fofu_III_I n.fofu_II_III n.isAugmentingPath_def)+
-
-      oops*)
-end
 end
