Original_Dinitz_Refine.thy
@@ -1,5 +1,5 @@
 theory Original_Dinitz_Refine
-  imports Original_Dinitz_Algo
+  imports Original_Dinitz_Algo Graph_Transpose
 begin
 text \<open>This theory takes the abstract definition of the Original Dinitz algorithm and refines
       it towards a concrete version. The goal here is not yet to arrive at an executable version,
@@ -140,95 +140,23 @@ proof (clarify, intro conjI)
     and "s \<notin> Q"
     and S_CON: "\<And>u v. connected s u \<Longrightarrow> Graph.connected c' s u \<and> c' (u, v) = c (u, v)"
     and NODE_HAS_IN: "\<forall>u \<in> Graph.V c' - Q - {s}. Graph.incoming c' u \<noteq> {}"
+    and "finite Q"
     unfolding rightPassInvar_def by auto
   then interpret Subgraph c' c by simp
-
-
-
-
-
-  interpret g': Graph c' .
   interpret g'': Graph c'' .
-
-  term g'.connected
-  term "Graph.connected c'"
-  term c'
-  term c
-  term c''
-  from INVAR have SUB: "Subgraph c' c" unfolding rightPassInvar_def by simp
-  from INVAR have SUB: "s \<notin> Q" unfolding rightPassInvar_def by simp
-  from INVAR have S_CON: "\<And>u v. connected s u \<Longrightarrow> g'.connected s u \<and> c' (u, v) = c (u, v)"
-
-
-  from INVAR have SUB: "Subgraph c' c"
-    and "s \<notin> Q"
-    and S_CON: "\<And>u v. connected s u \<Longrightarrow> g'.connected s u \<and> c' (u, v) = c (u, v)"
-    and NODE_HAS_IN: "\<forall>u \<in> g'.V - Q - {s}. g'.incoming  u \<noteq> {}"
-    unfolding rightPass_partial_invar_def by simp_all
-
-
-  oops
-
-
-  from T_INVAR have P_INVAR: "rightPass_partial_invar c s (c', Q)" and "finite Q"
-    unfolding rightPass_total_invar_def by auto
-  then interpret g': Finite_Graph c' unfolding rightPass_partial_invar_def Finite_Graph_def
-    using Subgraph.V_ss finite_V finite_subset by fast
-
-  from S_NO_IN \<open>u \<in> Q\<close> U_NO_IN P_INVAR show "rightPass_partial_invar c s (c'', Q')"
-    unfolding c''_def Q'_def by (rule rightPassRefine_partial_step)
-
-  from \<open>finite Q\<close> show "finite Q'" unfolding Q'_def by blast
-
-  show "((c'', Q'), c', Q) \<in> GraphWorkingSet_rel"
-  proof (cases "g'.outgoing u = {}")
-    case True
-    then have "c'' = c'" unfolding c''_def removeEdges_def by simp
-    moreover from True have "Q' = Q - {u}" unfolding Q'_def by simp
-    moreover note \<open>u \<in> Q\<close> \<open>finite Q\<close>
-    ultimately show ?thesis unfolding GraphWorkingSet_rel_def by auto
-  next
-    case False
-    then have "Proper_Subgraph c'' c'" unfolding c''_def
-      using g'.removeEdges_psg g'.outgoing_edges Proper_Subgraph.intro by blast
-    then show ?thesis unfolding GraphWorkingSet_rel_def finiteProperSubgraph_def
-      using g'.Finite_Graph_axioms by simp
-  qed
-qed
-
-(* TODO check use of c''_def / Q'_def *)
-lemma (in Graph) rightPassRefine_partial_step:
-  assumes S_NO_IN: "incoming s = {}"
-    and "u \<in> Q"
-    and U_NO_IN: "Graph.incoming c' u = {}"
-    and INVAR: "rightPass_partial_invar c s (c', Q)"
-  defines "c'' \<equiv> removeEdges c' (Graph.outgoing c' u)"
-    and "Q' \<equiv> Q - {u} \<union> snd ` Graph.outgoing c' u"
-  shows "rightPass_partial_invar c s (c'', Q')"
-  (*shows "rightPass_partial_invar c s (removeEdges c' (Graph.outgoing c' u), Q - {u} \<union> snd ` Graph.outgoing c' u)"
-    (is "rightPass_partial_invar c s (?c'', ?Q')")*)
-  unfolding rightPass_partial_invar_def
-proof (clarify, intro conjI)
-  interpret g': Graph c' .
-  interpret g'': Graph c'' .
-  from INVAR have SUB: "Subgraph c' c"
-    and "s \<notin> Q"
-    and S_CON: "\<And>u v. connected s u \<Longrightarrow> g'.connected s u \<and> c' (u, v) = c (u, v)"
-    and NODE_HAS_IN: "\<forall>u \<in> g'.V - Q - {s}. g'.incoming  u \<noteq> {}"
-    unfolding rightPass_partial_invar_def by simp_all
 
   show "Subgraph c'' c" unfolding c''_def
-    using g'.removeEdges_sg SUB subgraph.order_trans by blast
+    using Subgraph_axioms g'.deleteEdges_sg subgraph.order.trans by blast
 
   show "s \<notin> Q'"
   proof -
-    from S_NO_IN SUB have "g'.incoming s = {}" unfolding Graph.incoming_def
-      using Subgraph.E'_ss by fast
+    from S_NO_IN have "g'.incoming s = {}" unfolding Graph.incoming_def
+      using E'_ss by fast
     then have "s \<notin> snd ` g'.outgoing u" unfolding g'.incoming_def g'.outgoing_def by fastforce
     with \<open>s \<notin> Q\<close> show "?thesis" unfolding Q'_def by blast
   qed
 
-  show "(\<forall>v w. connected s v \<longrightarrow> g''.connected s v \<and> c'' (v, w) = c (v, w))"
+  show "\<forall>v w. connected s v \<longrightarrow> g''.connected s v \<and> c'' (v, w) = c (v, w)"
   proof (clarify, intro conjI)
     from \<open>u \<in> Q\<close> \<open>s \<notin> Q\<close> have "u \<noteq> s" by blast
     fix v w
@@ -239,12 +167,12 @@ proof (clarify, intro conjI)
       by (metis g'.distinct_nodes_have_in_out_if_connected(2) g'.connected_def g'.pathVertices_fwd g'.split_path_at_vertex)
     with PATH' have "g'.outgoing u \<inter> set p = {}"
       using g'.outgoing_edges_not_on_path g'.pathVertices_fwd by simp
-    with PATH' have "g''.isPath s p v" unfolding Graph.isPath_alt c''_def using g'.removeEdges_E by blast
+    with PATH' have "g''.isPath s p v" unfolding Graph.isPath_alt c''_def using g'.deleteEdges_E by blast
     then show "g''.connected s v" using g''.connected_def by blast
 
     from \<open>u \<noteq> s\<close> CON' U_NO_IN have "u \<noteq> v" using g'.distinct_nodes_have_in_out_if_connected(2) by blast
     then have "c'' (v, w) = c' (v, w)"
-      unfolding g'.outgoing_def removeEdges_def c''_def by simp
+      unfolding g'.outgoing_def deleteEdges_def c''_def by simp
     then show "c'' (v, w) = c (v, w)" using C'_EQ_C by simp
   qed
 
@@ -253,29 +181,45 @@ proof (clarify, intro conjI)
     fix v
     assume "v \<in> g''.V" "v \<noteq> s" "v \<notin> snd ` g'.outgoing u" "v \<in> Q \<longrightarrow> v = u" "g''.incoming v = {}"
     from \<open>v \<in> g''.V\<close> have "v \<in> g'.V" unfolding c''_def
-      using g'.removeEdges_sg Subgraph.V_ss by fast
+      using g'.deleteEdges_sg Subgraph.V_ss by fast
     have "v \<notin> Q"
     proof
       assume "v \<in> Q"
       with \<open>v \<in> Q \<longrightarrow> v = u\<close> have "v = u" by blast
       moreover from U_NO_IN have "g''.incoming u = {}" unfolding c''_def Graph.incoming_def
-        using g'.removeEdges_E by auto
+        using g'.deleteEdges_E by auto
       moreover note \<open>v \<in> g''.V\<close>
       ultimately obtain w where "(u, w) \<in> g''.E"
         unfolding g''.incoming_def by (auto elim: g''.vertex_cases)
-      then show False unfolding c''_def using g'.removeEdges_E g'.outgoing_alt by fastforce
+      then show False unfolding c''_def using g'.deleteEdges_E g'.outgoing_alt by fastforce
     qed
     with \<open>v \<in> g'.V\<close> \<open>v \<noteq> s\<close> NODE_HAS_IN obtain u' where "(u', v) \<in> g'.E" unfolding g'.incoming_def by blast
-    with \<open>v \<notin> snd ` g'.outgoing u\<close> have "(u', v) \<in> g''.E" unfolding c''_def using g'.removeEdges_E by blast
+    with \<open>v \<notin> snd ` g'.outgoing u\<close> have "(u', v) \<in> g''.E" unfolding c''_def using g'.deleteEdges_E by blast
     with \<open>g''.incoming v = {}\<close> show False unfolding g''.incoming_def by blast
+  qed
+
+  interpret g': Finite_Graph c' unfolding Finite_Graph_def
+    using V_ss finite_V finite_subset by blast
+
+  from \<open>finite Q\<close> show "finite Q'" unfolding Q'_def by blast
+
+  show "((Q', c''), Q, c') \<in> graphWorkingSetRel"
+  proof (cases "g'.outgoing u = {}")
+    case True
+    then have "c'' = c'" unfolding c''_def deleteEdges_def by simp
+    moreover from True have "Q' = Q - {u}" unfolding Q'_def by simp
+    moreover note \<open>u \<in> Q\<close> \<open>finite Q\<close>
+    ultimately show ?thesis unfolding graphWorkingSetRel_def by auto
+  next
+    case False
+    then have "Proper_Subgraph c'' c'" unfolding c''_def
+      using g'.removeEdges_psg g'.outgoing_edges Proper_Subgraph.intro by blast
+    then show ?thesis unfolding graphWorkingSetRel_def finiteProperSubgraph_def
+      using g'.Finite_Graph_axioms by simp
   qed
 qed
 
-context Distance_Bounded_Graph
-begin
-
-thm subgraph.order_antisym
-lemma rightPassRefine_final:
+lemma (in Distance_Bounded_Graph) rightPassRefine_final:
   assumes SUB: "Subgraph c' c"
     and S_CON: "\<And>u v. connected s u \<Longrightarrow> Graph.connected c' s u \<and> c' (u, v) = c (u, v)"
     and NODE_HAS_IN: "\<forall>u \<in> Graph.V c' - {s}. Graph.incoming c' u \<noteq> {}"
@@ -300,141 +244,774 @@ next
   finally show "right_pass s c (u, v) = c' (u, v)" by simp
 qed (* TODO cleanup *)
 
-theorem rightPassRefine_partial_correct:
-  assumes S_NO_IN: "incoming s = {}"
-    and Q_START: "s \<notin> Q" "\<forall>u \<in> V - Q - {s}. incoming u \<noteq> {}"
-  shows "rightPassRefine_partial Q c \<le> RETURN (right_pass s c)"
-  unfolding rightPassRefine_partial_def
-proof (intro WHILE_rule[where I="rightPass_partial_invar c s"] refine_vcg, clarsimp_all)
-  show "rightPass_partial_invar c s (c, Q)" unfolding rightPass_partial_invar_def using Q_START by blast
-next
-  fix c' Q u
-  assume step_assms: "rightPass_partial_invar c s (c', Q)" "u \<in> Q"
-  then show "Graph.incoming c' u \<noteq> {} \<Longrightarrow> rightPass_partial_invar c s (c', Q - {u})"
-    unfolding rightPass_partial_invar_def by blast
-
-  let ?c'' = "removeEdges c' (Graph.outgoing c' u)"
-  let ?Q' = "Q - {u} \<union> snd ` Graph.outgoing c' u"
-  from S_NO_IN step_assms show "Graph.incoming c' u = {} \<Longrightarrow> rightPass_partial_invar c s (?c'', ?Q')"
-    using rightPassRefine_partial_step by simp
-next
-  fix c'
-  assume "rightPass_partial_invar c s (c', {})"
-  then show "right_pass s c = c'" unfolding rightPass_partial_invar_def using rightPassRefine_final by simp
-qed
-end
-
-subsubsection \<open>Total correctness\<close>
-
-definition right_pass_refine :: "node set \<Rightarrow> _ graph \<Rightarrow> (_ graph) nres" where
-  "right_pass_refine Q c \<equiv> do {
-    (c, _) \<leftarrow> WHILE\<^sub>T (\<lambda>(_, Q). Q \<noteq> {}) (\<lambda>(c, Q). do {
-      u \<leftarrow> RES Q;
-      let Q = Q - {u};
-      if Graph.incoming c u = {} then do {
-        let R = Graph.outgoing c u;
-        let Q = Q \<union> (snd ` R);
-        let c = removeEdges c R;
-        RETURN (c, Q)}
-      else RETURN (c, Q)
-    }) (c, Q);
-    RETURN c
-  }"
-
-definition finiteProperSubgraph :: "_ graph rel"
-  where "finiteProperSubgraph \<equiv> {(c', c). Proper_Subgraph c' c \<and> Finite_Graph c}"
-
-lemma wf_finiteProperSubgraph: "wf finiteProperSubgraph"
-proof (rule wf_subset)
-  show "wf (inv_image finite_psubset Graph.E)" by simp
-  show "finiteProperSubgraph \<subseteq> inv_image finite_psubset Graph.E"
-    unfolding finiteProperSubgraph_def inv_image_def finite_psubset_def
-    using Proper_Subgraph.E'_pss Finite_Graph.finite_E by blast
-qed
-
-definition GraphWorkingSet_rel :: "(_ graph \<times> _ set) rel"
-  where "GraphWorkingSet_rel \<equiv> finiteProperSubgraph <*lex*> finite_psubset"
-
-lemma wf_GraphWorkingSet_rel: "wf GraphWorkingSet_rel" unfolding GraphWorkingSet_rel_def
-  using wf_finiteProperSubgraph by auto
-
-definition rightPass_total_invar :: "_ graph \<Rightarrow> node \<Rightarrow> (_ graph \<times> node set) \<Rightarrow> bool"
-  where "rightPass_total_invar c s \<equiv> \<lambda>(c', Q). rightPass_partial_invar c s (c', Q)
-                                \<and> finite Q"
-
-(* TODO does this make sense?
-interpretation subgraph: wellorder isSubgraph isProperSubgraph oops
-thm subgraph.wf
-*)
-
-
-lemma (in Finite_Graph) right_pass_refine_step:
-  assumes S_NO_IN: "incoming s = {}"
-    and "u \<in> Q"
-    and U_NO_IN: "Graph.incoming c' u = {}"
-    and T_INVAR: "rightPass_total_invar c s (c', Q)"
-  defines "c'' \<equiv> removeEdges c' (Graph.outgoing c' u)"
-    and "Q' \<equiv> Q - {u} \<union> snd ` Graph.outgoing c' u"
-  shows "rightPass_total_invar c s (c'', Q') \<and> ((c'', Q'), (c', Q)) \<in> GraphWorkingSet_rel"
-  unfolding rightPass_total_invar_def
-proof (clarify, intro conjI)
-  from T_INVAR have P_INVAR: "rightPass_partial_invar c s (c', Q)" and "finite Q"
-    unfolding rightPass_total_invar_def by auto
-  then interpret g': Finite_Graph c' unfolding rightPass_partial_invar_def Finite_Graph_def
-    using Subgraph.V_ss finite_V finite_subset by fast
-
-  from S_NO_IN \<open>u \<in> Q\<close> U_NO_IN P_INVAR show "rightPass_partial_invar c s (c'', Q')"
-    unfolding c''_def Q'_def by (rule rightPassRefine_partial_step)
-
-  from \<open>finite Q\<close> show "finite Q'" unfolding Q'_def by blast
-
-  show "((c'', Q'), c', Q) \<in> GraphWorkingSet_rel"
-  proof (cases "g'.outgoing u = {}")
-    case True
-    then have "c'' = c'" unfolding c''_def removeEdges_def by simp
-    moreover from True have "Q' = Q - {u}" unfolding Q'_def by simp
-    moreover note \<open>u \<in> Q\<close> \<open>finite Q\<close>
-    ultimately show ?thesis unfolding GraphWorkingSet_rel_def by auto
-  next
-    case False
-    then have "Proper_Subgraph c'' c'" unfolding c''_def
-      using g'.removeEdges_psg g'.outgoing_edges Proper_Subgraph.intro by blast
-    then show ?thesis unfolding GraphWorkingSet_rel_def finiteProperSubgraph_def
-      using g'.Finite_Graph_axioms by simp
-  qed
-qed
-
-context Finite_Bounded_Graph
-begin
-theorem right_pass_refine_correct:
+(* TODO remove right_pass, instead use locale *)
+theorem (in Finite_Bounded_Graph) rightPassRefine_correct:
   assumes S_NO_IN: "incoming s = {}"
     and Q_START: "s \<notin> Q" "\<forall>u \<in> V - Q - {s}. incoming u \<noteq> {}" "finite Q"
-  shows "right_pass_refine Q c \<le> RETURN (right_pass s c)"
-  unfolding right_pass_refine_def
-proof (intro WHILET_rule[where I="rightPass_total_invar c s"] refine_vcg, clarsimp_all)
-  show "wf GraphWorkingSet_rel" by (rule wf_GraphWorkingSet_rel)
+  shows "rightPassRefine Q c \<le> RETURN (right_pass s c)"
+  unfolding rightPassRefine_def
+proof (refine_vcg WHILET_rule[where I="rightPassInvar c s" and R=graphWorkingSetRel], clarsimp_all)
+  show "wf graphWorkingSetRel" by (rule wf_graphWorkingSetRel)
 next
-  show "rightPass_total_invar c s (c, Q)" unfolding rightPass_partial_invar_def rightPass_total_invar_def
-    using Q_START apply clarify (* TODO *) by blast
+  show "rightPassInvar c s (Q, c)" unfolding rightPassInvar_def using Q_START by fastforce
 next
   fix c' Q u
-  assume step_assms: "rightPass_total_invar c s (c', Q)" "u \<in> Q"
-  then show "Graph.incoming c' u \<noteq> {} \<Longrightarrow> rightPass_total_invar c s (c', Q - {u}) \<and> ((c', Q - {u}), (c', Q)) \<in> GraphWorkingSet_rel"
-    by (auto simp: rightPass_total_invar_def rightPass_partial_invar_def GraphWorkingSet_rel_def)
+  assume step_assms: "rightPassInvar c s (Q, c')" "u \<in> Q"
+  {
+    assume "Graph.incoming c' u \<noteq> {}"
+    with step_assms show "rightPassInvar c s (Q - {u}, c')" "((Q - {u}, c'), (Q, c')) \<in> graphWorkingSetRel"
+      by (auto simp: rightPassInvar_def graphWorkingSetRel_def)
+  }
 
-  let ?c'' = "removeEdges c' (Graph.outgoing c' u)"
+  let ?c'' = "deleteEdges c' (Graph.outgoing c' u)"
   let ?Q' = "Q - {u} \<union> snd ` Graph.outgoing c' u"
-  from S_NO_IN step_assms show "Graph.incoming c' u = {} \<Longrightarrow> rightPass_total_invar c s (?c'', ?Q') \<and> ((?c'', ?Q'), (c', Q)) \<in> GraphWorkingSet_rel"
-    using right_pass_refine_step by blast
+  assume "Graph.incoming c' u = {}"
+  with S_NO_IN step_assms show "rightPassInvar c s (?Q', ?c'')" "((?Q', ?c''), (Q, c')) \<in> graphWorkingSetRel"
+    using rightPassRefine_step by auto
 next
   fix c'
-  assume "rightPass_total_invar c s (c', {})"
-  then show "right_pass s c = c'" unfolding rightPass_total_invar_def rightPass_partial_invar_def
+  assume "rightPassInvar c s ({}, c')"
+  then show "right_pass s c = c'" unfolding rightPassInvar_def
     using rightPassRefine_final by simp
 qed
 
+\<comment> \<open>Right Pass\<close>
+
+subsubsection \<open>Left Pass\<close>
+text \<open>Used primitives:
+  - working set operation: adding elements, removing element, checking for emptiness
+  - graph operations: checking outgoing for emptiness, getting set of incoming edges
+  - delete_edges\<close>
+definition leftPassRefine :: "node set \<Rightarrow> _ graph \<Rightarrow> (_ graph) nres" where
+  "leftPassRefine Q c \<equiv> do {
+    (_, c) \<leftarrow> WHILE\<^sub>T
+      (\<lambda>(Q, _). Q \<noteq> {})
+      (\<lambda>(Q, c). do {
+        u \<leftarrow> RES Q;
+        let Q = Q - {u};
+        if Graph.outgoing c u = {}
+          then do {
+            let L = Graph.incoming c u;
+            let Q = Q \<union> (fst ` L);
+            let c = deleteEdges c L;
+            RETURN (Q, c)}
+          else RETURN (Q, c)})
+      (Q, c);
+    RETURN c
+  }"
+
+context Finite_Bounded_Graph
+begin
+interpretation Dual_Graph_Algorithms "leftPassRefine Q" "rightPassRefine Q"
+proof
+  fix c :: "('capacity::linordered_idom) graph"
+  note[refine_dref_RELATES] = RELATESI[of transpose_graph_rel]
+  show "leftPassRefine Q c \<le> \<Down> transpose_graph_rel (rightPassRefine Q (transpose_graph c))"
+    unfolding rightPassRefine_def leftPassRefine_def
+    apply refine_rcg
+    apply refine_dref_type
+    by (auto simp: transpose_graph_rel_def deleteEdges_def)
+
+  show "rightPassRefine Q c \<le> \<Down> transpose_graph_rel (leftPassRefine Q (transpose_graph c))"
+    unfolding rightPassRefine_def leftPassRefine_def
+    apply refine_rcg
+    apply refine_dref_type
+    by (auto simp: transpose_graph_rel_def deleteEdges_def)
+qed
+
+(* TODO cleanup proof *)
+theorem leftPassRefine_correct:
+  assumes T_NO_OUT: "outgoing t = {}"
+    and Q_START: "t \<notin> Q" "\<forall>u \<in> V - Q - {t}. outgoing u \<noteq> {}" "finite Q"
+  shows "leftPassRefine Q c \<le> RETURN (left_pass t c)"
+  apply (intro transfer_return[where ret'="right_pass t"])
+   apply (fastforce simp: right_pass_def left_pass_def)
+  apply (intro Finite_Bounded_Graph.rightPassRefine_correct)
+  using assms Finite_Bounded_Graph_axioms by (auto simp: converse_empty_simp)
+  (*by (metis converse_converse converse_empty)*)
 end
 
-\<comment> \<open>RightPass\<close>
+\<comment> \<open>Left Pass\<close>
 
+subsubsection \<open>Cleaning Algorithm\<close>
+
+definition cleaningRefine :: "node set \<Rightarrow> _ graph \<Rightarrow> (_ graph) nres" where
+  "cleaningRefine Q c \<equiv> do {
+    c \<leftarrow> rightPassRefine Q c;
+    c \<leftarrow> leftPassRefine Q c;
+    RETURN c}"
+
+lemma (in Finite_Bounded_Graph) cleaning_algo_correct:
+  assumes S_NO_IN: "incoming s = {}"
+    and T_NO_OUT: "outgoing t = {}"
+    and Q_START: "s \<notin> Q" "t \<notin> Q" "\<forall>u \<in> V - Q - {s, t}. incoming u \<noteq> {} \<and> outgoing u \<noteq> {}" "finite Q"
+  shows "cleaningRefine Q c \<le> RETURN (cleaning s t c)"
+  unfolding cleaningRefine_def
+proof (refine_vcg, simp)
+  from T_NO_OUT \<open>\<forall>u \<in> V - Q - {s, t}. incoming u \<noteq> {} \<and> outgoing u \<noteq> {}\<close> have "\<forall>u \<in> V - Q - {s}. incoming u \<noteq> {}"
+    by (cases "incoming t = {}") (auto simp: incoming_def outgoing_def V_def)
+  with assms have "rightPassRefine Q c \<le> RETURN (right_pass s c)"
+    by (blast intro: rightPassRefine_correct)
+  also have "... \<le> SPEC (\<lambda>ca. leftPassRefine Q ca \<le> RES {cleaning s t c})"
+  proof simp
+    interpret Subgraph "right_pass s c" c using right_pass_Subgraph .
+    have "leftPassRefine Q (right_pass s c) \<le> RETURN (left_pass t (right_pass s c))" (* TODO prettify *)
+      apply (intro Finite_Bounded_Graph.leftPassRefine_correct)
+          prefer 3 using assms apply simp
+         prefer 4 using assms apply simp
+        prefer 2 subgoal
+        using \<open>outgoing t = {}\<close>
+        unfolding Graph.outgoing_def Graph.E_def right_pass_def by simp
+      unfolding Finite_Bounded_Graph_def apply auto[1]
+      using edges_ss g'.Finite_Graph_EI rev_finite_subset apply blast
+      using Distance_Bounded_Graph_axioms apply (rule sg_Distance_Bounded)
+    proof
+      fix u
+      assume "u \<in> V' - Q - {t}"
+      then have "outgoing u \<noteq> {}" (* TODO prettify *)
+      proof (cases "outgoing s = {}")
+        case True
+        with S_NO_IN have "s \<notin> V" unfolding incoming_def outgoing_def V_def by blast
+        then have "s \<notin> V'" using V_ss by blast
+        with \<open>u \<in> V' - Q - {t}\<close> have "u \<noteq> s" by blast
+        with assms \<open>u \<in> V' - Q - {t}\<close> show ?thesis using V_ss by blast
+      next
+        case False
+        with \<open>u \<in> V' - Q - {t}\<close> show ?thesis using assms V_ss by auto
+      qed
+      then obtain v where "(u, v) \<in> E" by fast
+
+      from \<open>u \<in> V' - Q - {t}\<close> have "u \<in> V'" by blast
+      then have "connected s u" unfolding g'.V_def
+        using S_Graph.rp_edges_s_connected connected_append_edge edge'_if_edge by blast
+      with \<open>(u, v) \<in> E\<close> have "(u, v) \<in> E'"
+        using S_Graph.s_connected_edges_remain by blast
+      then show "g'.outgoing u \<noteq> {}" unfolding g'.outgoing_def by blast
+    qed
+    also have "... \<le> RES {cleaning s t c}"
+      by (simp add: ST_Graph.left_right_pass_is_cleaning)
+    finally show "leftPassRefine Q (right_pass s c) \<le> RES {cleaning s t c}" .
+  qed
+  finally show "rightPassRefine Q c \<le> SPEC (\<lambda>ca. leftPassRefine Q ca \<le> RES {cleaning s t c})" .
+qed
+
+\<comment> \<open>Cleaning Algorithm\<close>
+
+\<comment> \<open>Cleaning\<close>
+
+
+
+
+
+
+
+
+
+
+
+
+
+
+
+
+
+
+
+
+
+
+
+
+
+
+
+
+
+
+
+
+subsection \<open>Dinitz phase refinement\<close>
+context Graph
+begin
+(* TODO bounded version *)
+definition build_st_layering :: "node \<Rightarrow> node \<Rightarrow> _ graph nres" where
+  "build_st_layering s t \<equiv> do {
+    sl \<leftarrow> ebfs s;
+    stl \<leftarrow> Graph.back_ebfs sl t;
+    RETURN stl
+  }"
+end
+
+(* TODO is Finite_Graph really what we want? *)
+context Finite_Graph
+begin
+lemma build_st_layering_correct:
+  "build_st_layering s t \<le> (spec c'. Dual_Shortest_Path_Union c' c s t)"
+  unfolding build_st_layering_def
+proof (refine_vcg, simp)
+  have "reachableNodes s \<subseteq> V \<union> {s}"
+    using Graph.distinct_nodes_in_V_if_connected(2) reachableNodes_def by auto
+  then have "finite (reachableNodes s)" using finite_V by (simp add: finite_subset)
+  then have "ebfs s \<le> (spec sl. Source_Shortest_Path_Union sl c s V)" by (rule ebfs_correct)
+  also have "... \<le> (spec sl. Graph.back_ebfs sl t \<le> (spec c'. Dual_Shortest_Path_Union c' c s t))"
+  proof (rule SPEC_rule)
+    fix c'
+    assume "Source_Shortest_Path_Union c' c s V"
+    then interpret Source_Shortest_Path_Union c' c s V .
+
+    have "{u. g'.connected u t} \<subseteq> V' \<union> {t}"
+      using g'.distinct_nodes_in_V_if_connected by auto
+    then have "finite {u. g'.connected u t}" using finite_V V_ss by (simp add: finite_subset)
+    then have "g'.back_ebfs t \<le> (spec c''. Target_Shortest_Path_Union c'' c' V' t)"
+      by (rule g'.back_ebfs_correct)
+    also from \<open>Source_Shortest_Path_Union c' c s V\<close> have "... \<le> (spec c''. Dual_Shortest_Path_Union c'' c s t)"
+      using SPEC_rule ST_SPU_dualI by metis
+    finally show "g'.back_ebfs t \<le> (spec c''. Dual_Shortest_Path_Union c'' c s t)" .
+  qed
+  finally show "ebfs s \<le> (spec sl. Graph.back_ebfs sl t \<le> (spec c'. Dual_Shortest_Path_Union c' c s t))" .
+qed
+
+end
+
+
+
+
+(* TODO *)
+end
+
+
+
+context NFlow
+begin
+
+section \<open>Experiment\<close>
+definition test1 :: "_ flow nres" where
+  "test1 \<equiv> do {
+    (f', _, _) \<leftarrow> WHILE\<^sub>T
+      (\<lambda>(_, _, brk). \<not> brk)
+      (\<lambda>(f', stl, _). do {
+            stl \<leftarrow> Graph.subtract_path_algo stl [(0, 0)];
+            RETURN (f', stl, False)
+          })
+      (f, c, False);
+    RETURN f'}"
+definition test2 :: "_ flow nres" where
+  "test2 \<equiv> do {
+    (f', _, _) \<leftarrow> WHILE\<^sub>T
+      (\<lambda>(_, _, brk). \<not> brk)
+      (\<lambda>(f', stl, _). do {
+            stl \<leftarrow> return (Graph.subtract_path stl [(0, 0)]);
+            RETURN (f', stl, False)
+          })
+      (f, c, False);
+    RETURN f'}"
+
+thm refine_dref_pattern
+(* TODO find out which rule leads to the spec term, which in turn means dref_type cannot infer relation type *)
+lemma "test1 \<le> \<Down> Id test2"
+  unfolding test1_def test2_def
+  apply refine_rcg
+         apply refine_dref_type
+      apply clarsimp_all
+  oops
+\<comment> \<open>Experiment\<close>
+
+
+
+
+
+(* TODO *)
+(*declare fun_relI[refine del]*)
+lemma RELATESI_workaround[refine_dref_pattern]:
+  "RELATES R \<Longrightarrow> S \<le> (spec x. (x, y) \<in> R) \<Longrightarrow> S \<le> (spec x. (x, y) \<in> R)" .
+
+
+thm build_st_layering_correct
+  Dual_Layer_Graph.greedyPathFinding_correct
+  subtract_path_algo_correct
+  Graph.inner_path_vertices_algo_correct
+  Finite_Bounded_Graph.cleaning_algo_correct
+
+(* TODO cleanup assertions *)
+
+(*
+definition dinitz_phase_assert_invar :: "(_ flow \<times> _ graph \<times> bool) \<Rightarrow> bool" where
+  "dinitz_phase_assert_invar \<equiv> \<lambda>(f', stl, brk).
+    NFlow c s t f'
+    \<and> Bounded_ST_Shortest_Path_Union stl (cf_of f') s t (cf.min_dist s t)
+    \<and> (Graph.connected (cf_of f') s t \<longrightarrow> cf.min_dist s t \<le> Graph.min_dist (cf_of f') s t)
+    \<and> (brk \<longrightarrow> \<not> Graph.connected stl s t)"
+
+definition dinitz_phase_assert :: "_ flow nres" where
+  "dinitz_phase_assert \<equiv> do {
+    stl \<leftarrow> (spec c'. ST_Shortest_Path_Union c' cf s t);
+    (f', _, _) \<leftarrow> WHILE\<^sub>T\<^bsup>dinitz_phase_assert_invar\<^esup>
+      (\<lambda>(_, _, brk). \<not> brk)
+      (\<lambda>(f', stl, _). do {
+        p' \<leftarrow> select p. Graph.isPath stl s p t;
+        case p' of
+          None \<Rightarrow> RETURN (f', stl, True)
+        | Some p \<Rightarrow> do {
+            assert (Graph.isPath stl s p t);
+            assert (ST_Shortest_Path_Union stl (cf_of f') s t);
+            Q_ls \<leftarrow> return (tl (butlast (Graph.pathVertices s p)));
+            assert (set Q_ls = set (Graph.pathVertices s p) - {s, t});
+            stl' \<leftarrow> return (Graph.subtract_path stl p);
+            assert (Contained_Graph stl' stl \<and> Graph.E stl \<subseteq> Graph.E stl' \<union> set p);
+            stl' \<leftarrow> return (cleaning s t stl');
+            let f' = NFlow.augment c f' (NPreflow.augmentingFlow c f' p);
+            RETURN (f', stl', False)
+          }})
+      (f, stl, False);
+    RETURN f'}"
+*)
+
+definition dinitz_phase_assert_invar :: "(_ flow \<times> _ graph \<times> bool \<times> bool) \<Rightarrow> bool" where
+  "dinitz_phase_assert_invar \<equiv> \<lambda>(f', stl, brk, changed).
+    NFlow c s t f'
+    \<and> Bounded_ST_Shortest_Path_Union stl (cf_of f') s t (cf.min_dist s t)
+    \<and> (Graph.connected (cf_of f') s t \<longrightarrow> cf.min_dist s t \<le> Graph.min_dist (cf_of f') s t)
+    \<and> (brk \<longrightarrow> \<not> Graph.connected stl s t)
+    \<and> (val \<le> Flow.val c s f')
+    \<and> (changed \<longleftrightarrow> f' \<noteq> f)
+    \<and> (changed \<longrightarrow> cf.connected s t)" (* \<and> (changed \<and> brk \<longrightarrow> cf.connected s t)" *)
+
+(* TODO can this be simplified to just changed \<longleftrightarrow> val < val'? *)
+lemma dinitz_phase_assert_invar_alt:
+  "dinitz_phase_assert_invar = (\<lambda>(f', stl, brk, changed).
+    dinitz_phase_invar (f', stl)
+    \<and> (brk \<longrightarrow> \<not> Graph.connected stl s t)
+    \<and> (val \<le> Flow.val c s f')
+    \<and> (changed \<longleftrightarrow> f' \<noteq> f)
+    \<and> (changed \<longrightarrow> cf.connected s t))" (* TODO does this work? *)
+  unfolding dinitz_phase_invar_def dinitz_phase_assert_invar_def by simp
+
+definition dinitz_phase_assert :: "(_ flow \<times> bool) nres" where
+  "dinitz_phase_assert \<equiv> do {
+    stl \<leftarrow> (spec c'. ST_Shortest_Path_Union c' cf s t);
+    (f', _, _, changed) \<leftarrow> WHILE\<^sub>T\<^bsup>dinitz_phase_assert_invar\<^esup>
+      (\<lambda>(_, _, brk, _). \<not> brk)
+      (\<lambda>(f', stl, _, changed). do {
+        p' \<leftarrow> select p. Graph.isPath stl s p t;
+        case p' of
+          None \<Rightarrow> RETURN (f', stl, True, changed)
+        | Some p \<Rightarrow> do {
+            assert (Graph.isPath stl s p t);
+            assert (ST_Shortest_Path_Union stl (cf_of f') s t);
+            Q_ls \<leftarrow> return (tl (butlast (Graph.pathVertices s p)));
+            assert (set Q_ls = set (Graph.pathVertices s p) - {s, t});
+            stl' \<leftarrow> return (Graph.subtract_path stl p);
+            assert (Contained_Graph stl' stl \<and> Graph.E stl \<subseteq> Graph.E stl' \<union> set p);
+            stl' \<leftarrow> return (cleaning s t stl');
+            let f' = NFlow.augment c f' (NPreflow.augmentingFlow c f' p);
+            RETURN (f', stl', False, True)
+          }})
+      (f, stl, False, False);
+    RETURN (f', changed)}"
+
+(* TODO comment about val needed for changed inequality *)
+
+(* TODO use this in phase step *)
+lemma stu_if_invar_and_path:
+  assumes INVAR: "dinitz_phase_invar (f', stl)"
+    and PATH: "Graph.isPath stl s p t"
+  shows "ST_Shortest_Path_Union stl (cf_of f') s t"
+proof -
+  from INVAR interpret f': NFlow c s t f' unfolding dinitz_phase_invar_def by blast
+
+  have BOUND_EQ: "cf.min_dist s t = f'.cf.min_dist s t"
+  proof -
+    from INVAR interpret Bounded_ST_Shortest_Path_Union stl f'.cf s t "cf.min_dist s t"
+      unfolding dinitz_phase_invar_def by simp
+    show ?thesis
+    proof (intro antisym)
+      from PATH INVAR show "cf.min_dist s t \<le> f'.cf.min_dist s t"
+        unfolding dinitz_phase_invar_def Graph.connected_def
+        using sg_paths_are_base_paths by blast
+      from PATH show "f'.cf.min_dist s t \<le> cf.min_dist s t" (* TODO fix proof *)
+      using f'.cf.isShortestPath_min_dist_def path_length_bounded shortest_path_transfer (* by simp *)
+      by (metis Bounded_Shortest_Path_Union.obtain_close_ST Bounded_Shortest_Path_Union_axioms emptyE g'.isEmpty_def g'.isPath_bwd_cases min_dist_transfer s_in_V_if_nonempty singleton_iff t_not_s)
+    qed
+  qed
+  with INVAR show "ST_Shortest_Path_Union stl (f'.cf) s t"
+    unfolding dinitz_phase_invar_def using min_st_dist_bound by fastforce
+qed
+
+lemma dinitz_phase_assert_step:
+  fixes f' stl changed
+  assumes PATH: "Graph.isPath stl s p t"
+      and INVAR: "dinitz_phase_assert_invar (f', stl, False, changed)"
+  defines "aug_f' \<equiv> NFlow.augment c f' (NPreflow.augmentingFlow c f' p)"
+      and "stl' \<equiv> cleaning s t (Graph.subtract_path stl p)"
+    shows "dinitz_phase_assert_invar (aug_f', stl', False, True) \<and> Graph.E stl' \<subset> Graph.E stl \<and> finite (Graph.E stl)"
+proof -
+  have "Flow.val c s f' < Flow.val c s aug_f'"
+  proof -
+    from INVAR interpret f': NFlow c s t f' unfolding dinitz_phase_assert_invar_def by blast
+    from INVAR PATH interpret stu: ST_Shortest_Path_Union stl "cf_of f'" s t
+      unfolding dinitz_phase_assert_invar_alt using stu_if_invar_and_path by blast
+
+    have "Flow f'.cf s t (f'.augmentingFlow p)"
+      apply (intro f'.augFlow_resFlow)
+      unfolding f'.isAugmentingPath_def
+      using PATH f'.cf.isShortestPath_alt stu.shortest_path_transfer by blast
+    moreover have "0 < Flow.val f'.cf s (f'.augmentingFlow p)"
+      by (simp add: Graph.shortestPath_is_path Graph.shortestPath_is_simple PATH f'.augFlow_val f'.isAugmentingPath_def f'.resCap_gzero_aux stu.shortest_path_transfer)
+    ultimately show ?thesis unfolding aug_f'_def using f'.augment_flow_value by simp
+  qed
+  with PATH INVAR show ?thesis unfolding dinitz_phase_assert_invar_alt aug_f'_def stl'_def
+    using dinitz_phase_step (* TODO prettify *)
+    apply auto
+    apply (meson Graph.connected_def ST_Shortest_Path_Union.st_connected_iff stu_if_invar_and_path)
+    by blast+
+qed
+
+
+
+
+definition "dinitz_phase_assert_wf_rel \<equiv> inv_image
+  (less_than_bool <*lex*> finite_psubset)
+  (\<lambda>(_, stl, brk, _). (\<not>brk, Graph.E stl))"
+
+
+find_theorems Graph.E Graph.subtract_path
+find_theorems Graph.E Graph.subtract_graph
+thm Graph.subtract_graph_untouched_edges
+
+lemma dinitz_phase_assert_correct:
+  "dinitz_phase_assert \<le> SPEC (\<lambda>(f', changed). res_dist_increasing_flow f' \<and> changed = (f' \<noteq> f) \<and> (changed \<longrightarrow> cf.connected s t))"
+  unfolding dinitz_phase_assert_def
+  apply (refine_vcg WHILEIT_rule[where R=dinitz_phase_assert_wf_rel])
+                      apply (all \<open>(clarsimp; fail)?\<close>)
+            apply (simp add: dinitz_phase_assert_wf_rel_def wf_lex_prod)
+            apply (simp add: dinitz_phase_assert_invar_def NFlow_axioms min_st_dist_bound)
+           defer defer defer
+  apply (simp add: Graph.subtract_path_alt) using Graph.subtract_graph_untouched_edges apply (metis (no_types, lifting) Graph.isPath_alt Graph.path_induced_graph_edges Int_Un_eq(4) Int_absorb1 Int_commute Un_Diff_cancel2 cf.isPath.simps(1) set_eq_subset t_not_s)
+          apply (simp add: dinitz_phase_assert_step)
+          apply (simp add: dinitz_phase_assert_step dinitz_phase_assert_wf_rel_def)
+        apply (simp add: dinitz_phase_assert_invar_alt Graph.connected_def)
+       apply (simp add: dinitz_phase_assert_wf_rel_def)
+      apply (clarsimp simp: dinitz_phase_assert_invar_alt dinitz_phase_final)
+      apply (simp add: dinitz_phase_assert_invar_alt)
+  apply (clarsimp simp: dinitz_phase_assert_invar_alt)
+proof clarsimp_all oops
+  fix f' stl p changed
+  interpret cf': Graph "cf_of f'" .
+  assume INVAR: "dinitz_phase_assert_invar (f', stl, False, changed)" and PATH: "Graph.isPath stl s p t"
+  then show "ST_Shortest_Path_Union stl (cf_of f') s t"
+    unfolding dinitz_phase_assert_invar_alt using stu_if_invar_and_path by blast
+  then interpret ST_Shortest_Path_Union stl "cf_of f'" s t .
+
+  from INVAR interpret f': NFlow c s t f' unfolding dinitz_phase_assert_invar_def by blast
+  interpret g': Nonnegative_Graph stl
+    using f'.cf.Nonnegative_Graph_axioms sg_Nonnegative_Graph by blast
+  (* TODO replace this with a simple 'have', need some way to use sublocale relations *)
+  interpret subt_pos_cont: Pos_Contained_Graph "g'.subtract_path p" stl
+    unfolding g'.subtract_path_alt
+    using g'.path_induced_graph_pos_contained Pos_Contained_Graph.subtract_le_contained by blast
+  show "Contained_Graph (g'.subtract_path p ) stl" by intro_locales
+
+  from PATH have "pathVertices s p = s # (tl (pathVertices s p))"
+    by (simp add: Graph.pathVertices_fwd pathVertices_fwd_def)
+  moreover from PATH have "pathVertices s p = butlast (pathVertices s p) @ [t]"
+    by (metis Graph.isPath_bwd_cases Graph.isPath_tail Graph.pathVertices_alt snoc_eq_iff_butlast' t_not_s)
+  ultimately have "pathVertices s p = s # (tl (butlast (pathVertices s p))) @ [t]"
+    by (metis butlast_tl empty_append_eq_id snoc_eq_iff_butlast' t_not_s tl_last)
+      (* TODO simplify, probably need to show s, t \<notin> tl (butlast (pathVertices s p)) *)
+  then show "set (tl (butlast (pathVertices s p))) = set (pathVertices s p) - {s, t}"
+    by (smt (verit, ccfv_threshold) Diff_insert0 Graph.isSimplePath_fwd Graph.pathVertices_fwd PATH Un_Diff_Int Un_insert_right distinct.simps(2) distinct_append empty_set insertCI insert_Diff1 list.simps(15) paths_are_simple set_append sup_bot.right_neutral)
+qed
+
+definition dinitz_phase_concrete :: "(_ flow \<times> bool) nres" where
+  "dinitz_phase_concrete \<equiv> do {
+    stl \<leftarrow> cf.build_st_layering s t;
+    (f', _, _, changed) \<leftarrow> WHILE\<^sub>T\<^bsup>dinitz_phase_assert_invar\<^esup>
+      (\<lambda>(_, _, brk, _). \<not> brk)
+      (\<lambda>(f', stl, _, changed). do {
+        p' \<leftarrow> Graph.greedy_st_path_finding stl s t;
+        case p' of
+          None \<Rightarrow> RETURN (f', stl, True, changed)
+        | Some p \<Rightarrow> do {
+            assert (Graph.isPath stl s p t);
+            assert (ST_Shortest_Path_Union stl (cf_of f') s t);
+            Q_ls \<leftarrow> inner_path_vertices_algo p;
+            assert (set Q_ls = set (Graph.pathVertices s p) - {s, t});
+            stl' \<leftarrow> Graph.subtract_path_algo stl p;
+            assert (Contained_Graph stl' stl \<and> Graph.E stl \<subseteq> Graph.E stl' \<union> set p);
+            stl' \<leftarrow> cleaning_algo (set Q_ls) stl';
+            let f' = NFlow.augment c f' (NPreflow.augmentingFlow c f' p);
+            RETURN (f', stl', False, True)
+          }})
+      (f, stl, False, False);
+    RETURN (f', changed)}"
+
+
+
+
+
+find_theorems Graph.pathVertices set
+find_theorems Graph.pathVertices_fwd set
+find_theorems Graph.pathVertices
+thm Graph.pathVertices_append
+
+(*
+lemma (in Graph) aux: "u \<notin> set (pathVertices s p) \<Longrightarrow> (u, v) \<notin> set p"
+  by (induction p arbitrary: s) auto(*TODO*)
+lemma (in Graph) aux2: "u \<notin> set (pathVertices s p) \<Longrightarrow> (v, u) \<notin> set p"
+  apply (induction p arbitrary: s)
+   apply simp
+  apply simp sledgehammer
+  apply (induction p arbitrary: s rule: rev_induct)
+   apply simp
+  apply (simp add: Graph.pathVertices_append) apply auto
+  by (induction p arbitrary: s) auto(*TODO*)*)
+
+
+
+lemma dinitz_phase_concrete_refine: "dinitz_phase_concrete \<le> \<Down> Id dinitz_phase_assert"
+  unfolding dinitz_phase_concrete_def dinitz_phase_assert_def
+  apply refine_rcg
+            apply refine_dref_type
+           apply clarsimp_all
+  using cf.build_st_layering_correct apply simp
+proof -
+  fix f' stl changed
+  assume "dinitz_phase_assert_invar (f', stl, False, changed)"
+  then interpret bstu: Bounded_ST_Shortest_Path_Union stl "cf_of f'" s t "cf.min_dist s t"
+    unfolding dinitz_phase_assert_invar_def by blast
+  show "Graph.greedy_st_path_finding stl s t \<le> (select p. Graph.isPath stl s p t)"
+    using bstu.greedy_st_path_finding_correct .
+next
+  fix f' stl p
+  assume "ST_Shortest_Path_Union stl (cf_of f') s t"
+  then interpret stu: ST_Shortest_Path_Union stl "cf_of f'" s t .
+
+  assume "Graph.isPath stl s p t"
+  then have SP: "Graph.isPath stl s p t" by blast
+  
+  show "inner_path_vertices_algo p \<le> RES {tl (butlast (Graph.pathVertices s p))}"
+    using inner_path_vertices_algo_correct by (simp add: RES_sng_eq_RETURN)
+
+  from SP show "Graph.subtract_path_algo stl p \<le> RES {Graph.subtract_path stl p}"
+    using stu.g'.isSPath_distinct stu.paths_are_simple stu.g'.subtract_path_algo_correct
+    by (metis RES_sng_eq_RETURN)
+
+  thm Finite_Bounded_Graph.cleaning_algo_correct
+  fix stl'
+  assume "Contained_Graph stl' stl" "Graph.E stl \<subseteq> Graph.E stl' \<union> set p"
+  show "cleaning_algo (set (Graph.pathVertices s p) - {s, t}) stl' \<le> RES {cleaning s t stl'}"
+  proof (unfold RES_sng_eq_RETURN, intro Finite_Bounded_Graph.cleaning_algo_correct)
+    show "s \<notin> set (Graph.pathVertices s p) - {s, t}"
+      "t \<notin> set (Graph.pathVertices s p) - {s, t}"
+      "finite (set (Graph.pathVertices s p) - {s, t})"
+      by auto
+    from \<open>Contained_Graph stl' stl\<close> show "Finite_Bounded_Graph stl' (stu.layer t)" unfolding Finite_Bounded_Graph_def
+      by (meson Finite_Graph.intro Graph.Efin_imp_Vfin Contained_Graph.edges_ss Contained_Graph.cont_Distance_Bounded cfE_of_finite infinite_super stu.Distance_Bounded_Graph_axioms stu.E'_ss)
+    from \<open>Contained_Graph stl' stl\<close> show "Graph.incoming stl' s = {}"
+      by (metis Graph.isShortestPath_min_dist_def SP Contained_Graph.cont_incoming_ss bot.extremum_uniqueI stu.b_length_paths_are_terminal(1) stu.path_is_shortest)
+      (*by (metis Subgraph.incoming_ss Subgraph_axioms incoming_s_empty subset_empty)*)
+    from \<open>Contained_Graph stl' stl\<close> show "Graph.outgoing stl' t = {}"
+      by (metis Diff_empty Diff_eq_empty_iff Graph.distinct_nodes_in_V_if_connected(2) Contained_Graph.cont_outgoing_ss stu.no_outgoingD stu.obtain_back_terminal_connected)
+      (*by (metis Subgraph.outgoing_ss Subgraph_axioms outgoing_t_empty subset_empty)*)
+    from \<open>Graph.E stl \<subseteq> Graph.E stl' \<union> set p\<close> show "\<forall>u\<in>Graph.V stl' - (set (Graph.pathVertices s p) - {s, t}) - {s, t}. Graph.incoming stl' u \<noteq> {} \<and> Graph.outgoing stl' u \<noteq> {}"
+    proof auto (* TODO *)
+      fix v
+      assume "v \<in> Graph.V stl'"
+      then have "v \<in> Graph.V stl" using Contained_Graph.vertices_ss[OF \<open>Contained_Graph stl' stl\<close>] by blast
+      moreover assume "v \<noteq> s" "v \<noteq> t"
+      ultimately obtain u w where IN_OUT: "(u, v) \<in> Graph.E stl" "(v, w) \<in> Graph.E stl"
+        by (metis Graph.isPath_bwd_cases Graph.isPath_fwd_cases stu.g'.connected_def stu.st_connected)
+      
+      assume "v \<notin> set (Graph.pathVertices s p)"
+      with \<open>Graph.isPath stl s p t\<close> have "v \<notin> set (Graph.pathVertices_fwd s p)"
+        by (simp add: stu.g'.pathVertices_fwd)
+      from IN_OUT have "(u, v) \<notin> set p" "(v, w) \<notin> set p" using stu.g'.adjacent_edges_not_on_path[OF \<open>Graph.isPath stl s p t\<close> \<open>v \<notin> set (Graph.pathVertices_fwd s p)\<close>]
+        unfolding stu.g'.adjacent_def stu.g'.incoming_def stu.g'.outgoing_def by auto
+      with \<open>Graph.E stl \<subseteq> Graph.E stl' \<union> set p\<close> IN_OUT have "(u, v) \<in> Graph.E stl'" "(v, w) \<in> Graph.E stl'" by auto
+      then show "Graph.incoming stl' v = {} \<Longrightarrow> False" "Graph.outgoing stl' v = {} \<Longrightarrow> False"
+        unfolding Graph.incoming_def Graph.outgoing_def by auto
+    qed
+  qed
+qed
+
+lemma dinitz_phase_concrete_correct: "dinitz_phase_concrete \<le> SPEC (\<lambda>(f', changed). res_dist_increasing_flow f' \<and> changed = (f' \<noteq> f) \<and> (changed \<longrightarrow> cf.connected s t))"
+  using dinitz_phase_concrete_refine dinitz_phase_assert_correct by simp
+end
+
+context Network
+begin
+(* TODO rework using changed flag *)
+definition dinitz_concrete :: "_ flow nres" where
+  "dinitz_concrete \<equiv> do {
+    (f, _) \<leftarrow> WHILE\<^sub>T snd (NFlow.dinitz_phase_concrete c s t \<circ> fst) (\<lambda>_. 0, True);
+    RETURN f}"
+
+(*
+definition dinitz_concrete_aux_rel where
+  "dinitz_concrete_aux_rel \<equiv> {((f, m), f)|f m. m \<or> isMaxFlow f}"
+term dinitz_concrete_aux_rel
+thm dinitz_concrete_aux_rel_def
+
+thm bind_refine
+lemma dinitz_concrete_refine: "dinitz_concrete \<le> \<Down> Id dinitz"
+  unfolding dinitz_concrete_def dinitz_def
+  apply (refine_rcg bind_refine[where R'=dinitz_concrete_aux_rel])
+  unfolding dinitz_concrete_aux_rel_def apply clarsimp_all
+  defer using NFlow.dinitz_phase_concrete_refine apply clarsimp
+*)
+find_consts "('a \<Rightarrow> bool) \<Rightarrow> ('b \<Rightarrow> bool) \<Rightarrow> 'a \<times> 'b \<Rightarrow> bool"
+term pred_prod
+
+
+theorem dinitz_concrete_correct: "dinitz_concrete \<le> SPEC (\<lambda>f. isMaxFlow f)"
+  unfolding dinitz_concrete_def
+  apply (refine_vcg WHILET_rule[where I="\<lambda>(f', m). NFlow c s t f' \<and> (m \<or> isMaxFlow f')"
+          and R="inv_image (less_than_bool <*lex*> res_dist_rel) prod.swap"])
+      apply (fastforce simp: res_dist_wf)
+     apply (clarsimp_all simp: NFlowI Network_axioms zero_is_flow)
+proof -
+  fix f
+  assume "NFlow c s t f"
+  then interpret NFlow c s t f .
+  have "dinitz_phase_concrete \<le> SPEC (\<lambda>(f', changed). res_dist_increasing_flow f' \<and> changed = (f' \<noteq> f) \<and> (changed \<longrightarrow> cf.connected s t))"
+    using dinitz_phase_concrete_correct .
+  also have "... \<le> (spec s'. (case s' of (f', m) \<Rightarrow> NFlow c s t f' \<and> (m \<or> isMaxFlow f')) \<and> (prod.swap s', True, f) \<in> less_than_bool <*lex*> res_dist_rel)"
+  proof (clarsimp, intro conjI)
+    fix f'
+    assume "res_dist_increasing_flow f'" and CON_IF_NEQ: "(f' \<noteq> f) \<longrightarrow> cf.connected s t"
+    then show "NFlow c s t f'"
+      unfolding res_dist_increasing_flow_def by simp
+    then interpret n': NFlow c s t f' .
+    from \<open>res_dist_increasing_flow f'\<close> have DIST: "n'.cf.connected s t \<longrightarrow> cf.min_dist s t < n'.cf.min_dist s t"
+      unfolding res_dist_increasing_flow_def by simp
+    with CON_IF_NEQ show "f' = f \<or> f' \<noteq> f \<and> (f', f) \<in> res_dist_rel" unfolding res_dist_rel_def by blast
+    from CON_IF_NEQ show "f' = f \<longrightarrow> isMaxFlow f"
+      using Graph.connected_def Graph.isSimplePath_fwd n'.fofu_III_I n'.fofu_II_III n'.isAugmentingPath_def DIST by blast
+  qed 
+  finally show "dinitz_phase_concrete \<le> (spec s'. (case s' of (f', m) \<Rightarrow> NFlow c s t f' \<and> (m \<or> isMaxFlow f')) \<and> (prod.swap s', True, f) \<in> less_than_bool <*lex*> res_dist_rel)" .
+qed
+
+(*
+term SPEC
+term "if changed then cf.connected s t \<and> res_dist_increasing_flow f' else \<not> cf.connected s t \<and> (f' = f))"
+lemma (in NFlow) dinitz_phase_concrete_correct_if:
+  "dinitz_phase_concrete \<le> SPEC (\<lambda>(f', changed).
+    (if changed then cf.connected s t \<and> res_dist_increasing_flow f' else \<not> cf.connected s t \<and> (f' = f)))"
+
+
+res_dist_increasing_flow f' \<and> changed = (cf.connected s t \<and> f' \<noteq> f))"
+  sorry*)
+
+
+
+(*
+term "inv_image (less_than_bool <*lex*> res_dist_rel) prod.swap"
+theorem dinitz_concrete_correct: "dinitz_concrete \<le> SPEC (\<lambda>f. isMaxFlow f)"
+  unfolding dinitz_concrete_def
+  apply (refine_vcg WHILET_rule[where I="\<lambda>(f', m). NFlow c s t f' \<and> (m \<or> isMaxFlow f')"
+          and R="inv_image (less_than_bool <*lex*> res_dist_rel) prod.swap"])
+      apply (fastforce simp: res_dist_wf)
+     apply (simp add: NFlowI Network_axioms zero_is_flow)
+    apply simp
+   defer apply simp
+
+proof clarsimp
+  fix f
+  assume "NFlow c s t f"
+  then interpret n: NFlow c s t f .
+  thm n.dinitz_phase_concrete_correct
+  have "n.dinitz_phase_concrete \<le> SPEC (\<lambda>(f', changed). n.res_dist_increasing_flow f' \<and> changed = (f' \<noteq> f))"
+    using n.dinitz_phase_concrete_correct .
+  also have "... \<le> (spec s'. (case s' of (f', m) \<Rightarrow> NFlow c s t f' \<and> (m \<or> isMaxFlow f')) \<and> (prod.swap s', True, f) \<in> less_than_bool <*lex*> res_dist_rel)"
+  proof (clarsimp, intro conjI)
+    fix f'
+    assume "n.res_dist_increasing_flow f'"
+    then show "NFlow c s t f'"
+      unfolding n.res_dist_increasing_flow_def by simp
+    then interpret n': NFlow c s t f' .
+    from \<open>n.res_dist_increasing_flow f'\<close> have DIST: "n'.cf.connected s t \<longrightarrow> n.cf.min_dist s t < n'.cf.min_dist s t"
+      unfolding n.res_dist_increasing_flow_def by simp
+
+    then show "NFlow c s t f' \<and> (f' = f \<longrightarrow> isMaxFlow f) \<and> (f' = f \<or> f' \<noteq> f \<and> (f', f) \<in> res_dist_rel)"
+      unfolding n.res_dist_increasing_flow_def apply auto
+        apply (meson Graph.connected_def Graph.isSimplePath_fwd n.ford_fulkerson(1) n.isAugmentingPath_def)
+      unfolding res_dist_rel_def apply auto oops
+
+
+      thm res_dist_rel_def
+
+theorem dinitz_concrete_correct: "dinitz_concrete \<le> SPEC (\<lambda>f. isMaxFlow f)"
+  unfolding dinitz_concrete_def
+  apply (refine_vcg WHILET_rule[where I="\<lambda>(f', m). NFlow c s t f' \<and> (m \<or> isMaxFlow f')"
+          and R="inv_image (less_than_bool <*lex*> res_dist_rel) prod.swap"])
+      apply (fastforce simp: res_dist_wf)
+     apply (simp add: NFlowI Network_axioms zero_is_flow)
+    apply simp
+   defer apply simp
+
+proof clarsimp
+  fix f
+  assume "NFlow c s t f"
+  then interpret n: NFlow c s t f .
+  thm n.dinitz_phase_concrete_correct'
+  have "n.dinitz_phase_concrete \<le> SPEC (\<lambda>(f', changed). n.res_dist_increasing_flow f' \<and> (changed \<longleftrightarrow> n.val < Flow.val c s f'))"
+    using n.dinitz_phase_concrete_correct' sorry
+  also have "... \<le> (spec s'. (case s' of (f', m) \<Rightarrow> NFlow c s t f' \<and> (m \<or> isMaxFlow f')) \<and> (prod.swap s', True, f) \<in> less_than_bool <*lex*> res_dist_rel)"
+  proof (clarsimp, intro conjI)
+    fix f'
+    assume "n.res_dist_increasing_flow f'"
+    then show "NFlow c s t f'"
+      unfolding n.res_dist_increasing_flow_def by simp
+    then interpret n': NFlow c s t f' .
+
+    from \<open>n.res_dist_increasing_flow f'\<close> have DIST: "n'.cf.connected s t \<longrightarrow> n.cf.min_dist s t < n'.cf.min_dist s t"
+      unfolding n.res_dist_increasing_flow_def by simp
+    then show "n.val < n'.val \<or> isMaxFlow f'" apply auto
+       apply (simp add: n'.ford_fulkerson(1) Graph.connected_def Graph.isSimplePath_fwd n'.isAugmentingPath_def)
+      sorry
+
+    from DIST show "n.val < n'.val \<longrightarrow> (f', f) \<in> res_dist_rel"
+      unfolding res_dist_rel_def
+      apply auto
+      by (meson Graph.connected_def Graph.isSimplePath_fwd isMaxFlow_def less_le_not_le n'.Flow_axioms n.fofu_III_I n.fofu_II_III n.isAugmentingPath_def)+
+
+    oops
+
+theorem dinitz_concrete_correct: "dinitz_concrete \<le> SPEC (\<lambda>f. isMaxFlow f)"
+  unfolding dinitz_concrete_def
+  apply (refine_vcg WHILET_rule[where I="\<lambda>(f', m). NFlow c s t f' \<and> (m \<or> isMaxFlow f')"
+          and R="inv_image (less_than_bool <*lex*> res_dist_rel) prod.swap"])
+      apply (fastforce simp: res_dist_wf)
+     apply (simp add: NFlowI Network_axioms zero_is_flow)
+    apply simp
+   defer apply simp
+
+proof clarsimp
+  fix f
+  assume "NFlow c s t f"
+  then interpret n: NFlow c s t f .
+  thm n.dinitz_phase_concrete_correct'
+  have "n.dinitz_phase_concrete \<le> SPEC (\<lambda>(f', changed). n.res_dist_increasing_flow f' \<and> (changed \<or> f' = f \<and> isMaxFlow f))"
+    using n.dinitz_phase_concrete_correct' .
+  also have "... \<le> (spec s'. (case s' of (f', m) \<Rightarrow> NFlow c s t f' \<and> (m \<or> isMaxFlow f')) \<and> (prod.swap s', True, f) \<in> less_than_bool <*lex*> res_dist_rel)"
+  proof (clarsimp, intro conjI)
+    fix f'
+    assume "n.res_dist_increasing_flow f'"
+    then show "NFlow c s t f'"
+      unfolding n.res_dist_increasing_flow_def by simp
+    then interpret n': NFlow c s t f' .
+
+    from \<open>n.res_dist_increasing_flow f'\<close> have DIST: "n'.cf.connected s t \<longrightarrow> n.cf.min_dist s t < n'.cf.min_dist s t"
+      unfolding n.res_dist_increasing_flow_def by simp
+    then show "n.val < n'.val \<or> isMaxFlow f'" apply auto
+       apply (simp add: n'.ford_fulkerson(1) Graph.connected_def Graph.isSimplePath_fwd n'.isAugmentingPath_def)
+      sorry
+
+    from DIST show "n.val < n'.val \<longrightarrow> (f', f) \<in> res_dist_rel"
+      unfolding res_dist_rel_def
+      apply auto
+      by (meson Graph.connected_def Graph.isSimplePath_fwd isMaxFlow_def less_le_not_le n'.Flow_axioms n.fofu_III_I n.fofu_II_III n.isAugmentingPath_def)+
+
+      oops*)
+end
 end
